finished proof and added documentation

TaskinBA/Complement/Complement_DPDA.thy
@@ -1,6 +1,148 @@
+section \<open>Closure Property of DCFLs under Complementation\<close>
+
 theory Complement_DPDA
   imports Det_Pushdown_Automata
 begin
+
+subsection \<open>Setup and Auxiliary Lemmas\<close>
+
+context pda begin
+
+definition stepst :: "'q \<times> 'a list \<times> 's list \<Rightarrow> 'q \<times> 'a list \<times> 's list \<Rightarrow> bool"
+  ("(_ \<leadsto>+ _)" [50, 50] 50) where
+  "stepst \<equiv> step\<^sub>1 ^++"
+
+abbreviation nstep\<^sub>1 ("(_ \<leadsto>)" [50] 50) where
+  "cf \<leadsto> \<equiv> (\<forall>cf'. \<not>cf \<leadsto> cf')"
+
+abbreviation nstepsn ("(_ /\<leadsto>'(_'))" [50, 0] 50) where
+  "cf \<leadsto>(n) \<equiv> (\<forall>cf'. \<not>cf \<leadsto>(n) cf')"
+
+lemma stepst_induct2[consumes 1]:
+  assumes "x1 \<leadsto>+ x2"
+      and "\<And>q w \<alpha> p u \<gamma>. (q, w, \<alpha>) \<leadsto> (p, u, \<gamma>) \<Longrightarrow> P (q, w, \<alpha>) (p, u, \<gamma>)"
+      and "\<And>q w \<alpha> r v \<beta> p u \<gamma>. (q, w, \<alpha>) \<leadsto> (r, v, \<beta>) \<Longrightarrow> (r, v, \<beta>) \<leadsto>+ (p, u, \<gamma>) \<Longrightarrow> 
+                P (r, v, \<beta>) (p, u, \<gamma>) \<Longrightarrow> P (q, w, \<alpha>) (p, u, \<gamma>)"
+    shows "P x1 x2"
+using assms[unfolded stepst_def]
+proof(induction rule: converse_tranclp_induct)
+  case base thus ?case by (metis prod_cases3)
+next
+  case step thus ?case by simp (metis prod_cases3 step\<^sub>1.simps)
+qed
+
+lemma stepst_induct2_bw[consumes 1, case_names base step]:
+  assumes "x1 \<leadsto>+ x2"
+      and "\<And>q w \<alpha> p u \<gamma>. (q, w, \<alpha>) \<leadsto> (p, u, \<gamma>) \<Longrightarrow> P (q, w, \<alpha>) (p, u, \<gamma>)"
+      and "\<And>q w \<alpha> r v \<beta> p u \<gamma>. (q, w, \<alpha>) \<leadsto>+ (r, v, \<beta>) \<Longrightarrow> (r, v, \<beta>) \<leadsto> (p, u, \<gamma>) \<Longrightarrow> 
+                P (q, w, \<alpha>) (r, v, \<beta>) \<Longrightarrow> P (q, w, \<alpha>) (p, u, \<gamma>)"
+    shows "P x1 x2"
+  using assms[unfolded stepst_def]
+proof(induction rule: tranclp_induct)
+  case base
+  then show ?case by (metis prod_cases3)
+next
+  case (step)
+  then show ?case by simp (metis prod_cases3 step\<^sub>1.simps)
+qed
+
+lemma stepst_steps:
+  "(q, w, \<alpha>) \<leadsto>+ (p, u, \<gamma>) \<Longrightarrow> (q, w, \<alpha>) \<leadsto>* (p, u, \<gamma>)"
+  by (simp add: steps_def stepst_def)
+
+lemma stepst_step:
+  "(q, w, \<alpha>) \<leadsto> (p, u, \<gamma>) \<Longrightarrow> (q, w, \<alpha>) \<leadsto>+ (p, u, \<gamma>)"
+  by (simp add: stepst_def tranclp.r_into_trancl)
+
+lemma stepst_trans:
+  "(q, w, \<alpha>) \<leadsto>+ (p, u, \<gamma>) \<Longrightarrow> (p, u, \<gamma>) \<leadsto>+ (r, v, \<beta>) \<Longrightarrow> (q, w, \<alpha>) \<leadsto>+ (r, v, \<beta>)"
+using stepst_def by force
+
+lemma steps_stepst:
+  assumes "(q, w, \<alpha>) \<leadsto>* (p, u, \<gamma>)"
+      and "(q, w, \<alpha>) \<noteq> (p, u, \<gamma>)"
+    shows "(q, w, \<alpha>) \<leadsto>+ (p, u, \<gamma>)"
+using assms unfolding steps_def stepst_def by (meson rtranclpD)
+
+lemma stepst_split_last: "(\<exists>r v \<beta>. (q, w, \<alpha>) \<leadsto>* (r, v, \<beta>) \<and> (r, v, \<beta>) \<leadsto> (p, u, \<gamma>)) 
+                                \<longleftrightarrow> (q, w, \<alpha>) \<leadsto>+ (p, u, \<gamma>)"
+proof
+  assume "\<exists>r v \<beta>. (q, w, \<alpha>) \<leadsto>* (r, v, \<beta>) \<and> (r, v, \<beta>) \<leadsto> (p, u, \<gamma>)"
+  then obtain r v \<beta> where "(q, w, \<alpha>) \<leadsto>* (r, v, \<beta>)" and "(r, v, \<beta>) \<leadsto> (p, u, \<gamma>)" by blast
+  then show "(q, w, \<alpha>) \<leadsto>+ (p, u, \<gamma>)"
+    by (simp add: steps_def stepst_def rtranclp_into_tranclp1)
+next
+  assume "(q, w, \<alpha>) \<leadsto>+ (p, u, \<gamma>)"
+  then show "\<exists>r v \<beta>. (q, w, \<alpha>) \<leadsto>* (r, v, \<beta>) \<and> (r, v, \<beta>) \<leadsto> (p, u, \<gamma>)"
+    by (induction rule: stepst_induct2_bw) (use steps_refl stepst_steps in blast)+
+qed
+
+lemma split_path:
+  assumes "(q, w, \<alpha>) \<leadsto>(n) (p, [], \<gamma>)"
+      and "m \<le> n"
+    shows "\<exists>r u \<beta>. (q, w, \<alpha>) \<leadsto>(m) (r, u, \<beta>) \<and> (r, u, \<beta>) \<leadsto>(n-m) (p, [], \<gamma>)"
+using assms proof (induction "n-m" arbitrary: m)
+  case (Suc x)
+  from Suc.prems(2) consider (a) "m=n" | (b) "m<n" by linarith
+  then show ?case
+  proof cases
+    case a
+    with Suc.prems(1) show ?thesis by auto
+  next
+    case b
+    with Suc.hyps(1)[of "Suc m"] Suc.hyps(2) Suc.prems(1) obtain r u \<beta>
+      where p1: "(q, w, \<alpha>) \<leadsto>(Suc m) (r, u, \<beta>)" and p2: "(r, u, \<beta>) \<leadsto>(n - Suc m) (p, [], \<gamma>)" by fastforce
+    from p1 obtain s v \<zeta> where *: "(q, w, \<alpha>) \<leadsto>(m) (s, v, \<zeta>)" and s: "(s, v, \<zeta>) \<leadsto> (r, u, \<beta>)"
+      using stepn_split_last[of m q w \<alpha> r u \<beta>] by auto
+    from s p2 b have **: "(s, v, \<zeta>) \<leadsto>(n - m) (p, [], \<gamma>)"
+      using stepn_split_first[of s v \<zeta> "n - Suc m" p "[]" \<gamma>] Suc_diff_Suc by force
+    from * ** show ?thesis by blast
+  qed
+qed auto
+
+end
+
+context dpda begin
+
+lemma max_eps_steps:
+  assumes "(q, w, \<alpha>) \<leadsto>(n) (p, u, \<gamma>)"
+      and "(p, [], \<gamma>) \<leadsto>"
+      and "(q, w, \<alpha>) \<leadsto>(m) (r, u, \<beta>)"
+    shows "m \<le> n"
+proof (rule ccontr)
+  assume "\<not> m \<le> n"
+  then have n_less_m: "Suc n \<le> m" by simp
+  from assms(1) obtain v where w_def: "w = v@u"
+    using stepn_steps[of q w \<alpha> p u \<gamma>] decreasing_word[of q w \<alpha> p u \<gamma>] by blast
+  from assms(3)[unfolded w_def] have p: "(q, v, \<alpha>) \<leadsto>(m) (r, [], \<beta>)"
+    using stepn_word_app[of m q v \<alpha> r "[]" \<beta> u] by simp
+  obtain s y \<zeta> where *: "(q, v, \<alpha>) \<leadsto>(Suc n) (s, y, \<zeta>)"
+    using split_path[OF p n_less_m] by fastforce
+  from assms(1)[unfolded w_def] have **: "(q, v, \<alpha>) \<leadsto>(n) (p, [], \<gamma>)" 
+    using stepn_word_app[of n q v \<alpha> p "[]" \<gamma> u] by simp
+  from * ** have "(p, [], \<gamma>) \<leadsto> (s, y, \<zeta>)"
+    using stepn_split_last[of n q v \<alpha> s y \<zeta>] dpda_stepn_det[of n q v \<alpha> p "[]" \<gamma>] by metis
+  with assms(2) show False by simp
+qed
+
+end
+
+text \<open>In what follows, we show that the complement of a deterministic context-free language is also a 
+      deterministic context-free language. For this purpose, we construct a deterministic pushdown automaton 
+      that recognizes the complement language of a given deterministic pushdown automaton. The proof 
+      follows that of Hopcroft and Ullman\cite{hopcroftullman}. The construction is divided into two parts: First, construct an equivalent 
+      deterministic pushdown automaton that scans the entire input for all given input words, and then construct the automaton that recognizes the complement 
+      language out of this automaton.\<close>
+
+subsection \<open>Scan Construction\<close>
+
+text \<open>To scan the entire input, we address two complications: ensuring that every configuration has a possible step and that 
+      no configuration allows infinite epsilon steps. For the first problem, we introduce a new stack symbol to prevent the 
+      stack from becoming empty and a dead state that the automaton moves to when there are no possible steps. For the second 
+      problem, we introduce a new final state that the automaton moves to if an infinite number of epsilon steps pass through 
+      a final state; otherwise, the automaton moves to the dead state.\<close>
+
+subsubsection \<open>Definition\<close>
 
 datatype 'q st_extended = OST 'q | Q0' | D | F
 datatype 's sym_extended = OSYM 's | X0
@@ -27,8 +169,6 @@ qed
 locale dpda_scan = dpda M for M :: "('q :: finite, 'a :: finite, 's :: finite) pda" 
 begin
 
-text \<open>In the following we define a deterministic pushdown automata that scans the entire input according to Hopcroft and Ullman.\<close>
-
 definition scan_dpda_final_states :: "'q st_extended set" where
   "scan_dpda_final_states \<equiv> OST ` final_states M \<union> {F}"
 
@@ -40,10 +180,10 @@ fun scan_dpda_delta :: "'q st_extended \<Rightarrow> 'a \<Rightarrow> 's sym_ext
 | "scan_dpda_delta _ _ _ = {}"
 
 definition eps_nonfinal :: "'q \<Rightarrow> 's \<Rightarrow> bool" where
-  "eps_nonfinal q X \<equiv> (\<forall>i. \<exists>p \<alpha>. (q, [], [X]) \<leadsto>\<^sub>d(i) (p, [], \<alpha>) \<and> p \<notin> final_states M)"
+  "eps_nonfinal q X \<equiv> (\<forall>i. \<exists>p \<alpha>. (q, [], [X]) \<leadsto>(i) (p, [], \<alpha>) \<and> p \<notin> final_states M)"
 
 definition eps_final :: "'q \<Rightarrow> 's \<Rightarrow> bool" where
-  "eps_final q X \<equiv> (\<forall>i. \<exists>p \<alpha>. (q, [], [X]) \<leadsto>\<^sub>d(i) (p, [], \<alpha>)) \<and> (\<exists>i p \<alpha>. (q, [], [X]) \<leadsto>\<^sub>d(i) (p, [], \<alpha>) \<and> p \<in> final_states M)"
+  "eps_final q X \<equiv> (\<forall>i. \<exists>p \<alpha>. (q, [], [X]) \<leadsto>(i) (p, [], \<alpha>)) \<and> (\<exists>i p \<alpha>. (q, [], [X]) \<leadsto>(i) (p, [], \<alpha>) \<and> p \<in> final_states M)"
 
 fun scan_dpda_delta_eps :: "'q st_extended \<Rightarrow> 's sym_extended \<Rightarrow> ('q st_extended \<times> 's sym_extended list) set" where
   "scan_dpda_delta_eps Q0' X0 = {(OST (init_state M), [OSYM (init_symbol M), X0])}"
@@ -57,7 +197,9 @@ definition scan_dpda :: "('q st_extended, 'a, 's sym_extended) pda" where
   "scan_dpda \<equiv> \<lparr> init_state = Q0', init_symbol = X0, final_states = scan_dpda_final_states, 
                   delta = scan_dpda_delta, delta_eps = scan_dpda_delta_eps \<rparr>"
 
-text \<open>The pushdown automaton @{const scan_dpda} is indeed deterministic.\<close>
+subsubsection \<open>Determinism\<close>
+
+text \<open>The automaton @{const [source] scan_dpda} is deterministic:\<close>
 lemma dpda_scan_dpda: "dpda scan_dpda"
 proof (standard, goal_cases)
   case (1 p a Z)
@@ -83,12 +225,11 @@ next
           using \<delta>_nonempty[of q a X] by satx
         with c show False by satx
       qed
-      hence **: "(q, [], [X]) \<leadsto>\<^sub>d"
-        by (simp add: det_step_def the_elem_opt_def)
+      hence **: "(q, [], [X]) \<leadsto>" by simp 
       from ** have ***: "\<not>eps_final q X"
-        unfolding eps_final_def using det_step\<^sub>1_det_stepn_one[of q "[]" "[X]"] by fastforce
+        by (force simp: eps_final_def)
       from ** have ****: "\<not>eps_nonfinal q X"
-        unfolding eps_nonfinal_def using det_step\<^sub>1_det_stepn_one[of q "[]" "[X]"] by fastforce
+        by (force simp: eps_nonfinal_def)
       from * *** **** show "scan_dpda_delta_eps (OST q) (OSYM X) = {}" by simp
     qed
   qed simp_all
@@ -105,24 +246,24 @@ next
   then show ?case by (simp add: scan_dpda_def)
 qed
 
+subsubsection \<open>Equivalence\<close>
+
 sublocale scan: dpda scan_dpda
   using dpda_scan_dpda .
 
-text \<open>We abbreviate step definitions for @{const scan_dpda} with the sub-index s.\<close>
-
+text \<open>We abbreviate the definitions of @{const [source] scan_dpda} with sub-index s:\<close>
 notation scan.step\<^sub>1 ("(_ \<leadsto>\<^sub>s _)" [50, 50] 50)
-notation scan.steps ("(_ \<leadsto>\<^sub>s* _)" [50, 50] 50)    
+notation scan.steps ("(_ \<leadsto>\<^sub>s* _)" [50, 50] 50)
+notation scan.nstep\<^sub>1 ("(_ \<leadsto>\<^sub>s)" [50] 50)
                                                            
 abbreviation stack_with_X0 :: "'s list \<Rightarrow> 's sym_extended list" where 
   "stack_with_X0 \<alpha> \<equiv> map OSYM \<alpha> @ [X0]"
 
-text \<open>Forced steps of @{const scan_dpda}}\<close>
 lemma scan_dpda_first_step:
   assumes "(Q0', w, [X0]) \<leadsto>\<^sub>s (q, u, \<alpha>)"
   shows "q = OST (init_state M) \<and> u = w \<and> \<alpha> = [OSYM (init_symbol M), X0]"
   using assms scan.step\<^sub>1_rule by (simp add: scan_dpda_def)
 
-text \<open>Deduction from steps of @{const scan_dpda}}\<close>
 lemma scan_dpda_step_from_OST:
   assumes "(OST q, w, \<alpha>) \<leadsto>\<^sub>s (p, u, \<gamma>)"
   shows "(\<exists>p'. p = OST p') \<or> p = F \<or> p = D"
@@ -210,7 +351,6 @@ using assms proof (induction "(OST q, w, stack_with_X0 \<alpha>)" "(OST p, u, \<
     by (metis append.assoc map_append)
 qed blast
 
-text \<open>The original pushdown automaton can mimic the steps of @{const scan_dpda} assuming that it never leaves the old states.\<close>
 lemma scan_dpda_trans:
   assumes "(OST q, map OSYM \<alpha>) \<in> \<delta> scan_dpda (OST p) a (OSYM X)"
   shows "(q, \<alpha>) \<in> \<delta> M p a X"
@@ -264,6 +404,7 @@ proof -
     using scan_dpda_step by presburger
 qed
 
+text \<open>The original automaton can mimic the steps of the automaton @{const [source] scan_dpda} in the old states:\<close>
 lemma scan_dpda_stepsX0:
   assumes "(OST q, w, stack_with_X0 \<alpha>) \<leadsto>\<^sub>s* (OST p, u, stack_with_X0 \<gamma>)"
   shows "(q, w, \<alpha>) \<leadsto>* (p, u, \<gamma>)"
@@ -280,15 +421,13 @@ next
   from step(3)[OF r_def \<beta>_def] have *: "(q, w, \<alpha>) \<leadsto>* (r', u, \<beta>')" .
   have **: "(r', u, \<beta>') \<leadsto> (p, v, \<gamma>)"
     using scan_dpda_stepX0[OF step(2)[simplified r_def \<beta>_def]] .
-  from * ** show ?case
-    using step\<^sub>1_steps steps_trans by blast
-qed   
+  show ?case
+    using steps_trans[OF * step\<^sub>1_steps[OF **]] .
+qed     
 
-text \<open>Before we move onto the converse direction, we need a helper lemma stating that if the pair (q, X) forces a cycle then the remaining part of the
-      stack is irrelevant.\<close>    
-                            
+text \<open>If a pair of a state and a stack symbol allows infinite epsilon steps then the rest of the stack content stays untouched:\<close>
 lemma stack_cycle_drop:    
-  assumes "\<forall>i. \<exists>p \<alpha>. (q, [], [X]) \<leadsto>\<^sub>d(i) (p, [], \<alpha>)"
+  assumes "\<forall>i. \<exists>p \<alpha>. (q, [], [X]) \<leadsto>(i) (p, [], \<alpha>)"
       and "(q, [], X#\<gamma>) \<leadsto>* (r, [], \<beta>)"
     shows "\<exists>Y \<beta>'. \<beta> = Y # \<beta>' @ \<gamma> \<and> (q, [], [X]) \<leadsto>* (r, [], Y#\<beta>')"
 using assms(2) proof (induction "(q, [] :: 'a list, X#\<gamma>)" "(r, [] :: 'a list, \<beta>)" arbitrary: r \<beta> rule: steps_induct2_bw)  
@@ -306,20 +445,20 @@ next
     using step\<^sub>1_stack_drop[of p "[]" "Y # \<beta>'" \<gamma> r "[]" "\<beta>'' @ \<beta>'"] by simp 
   have *: "(q, [], [X]) \<leadsto>* (r, [], \<beta>'' @ \<beta>')"             
     using steps_trans[OF p1 step\<^sub>1_steps[OF p2]] .  
-  from * obtain n where d1: "(q, [], [X]) \<leadsto>\<^sub>d(n) (r, [], \<beta>'' @ \<beta>')"
-    using stepn_steps[of q "[]" "[X]" r "[]" "\<beta>'' @ \<beta>'"] stepn_det_stepn\<^sub>1[of _  q "[]" "[X]" r "[]" "\<beta>'' @ \<beta>'"] by blast
-  from assms(1) obtain s \<zeta> where d2: "(q, [], [X]) \<leadsto>\<^sub>d(Suc n) (s, [], \<zeta>)" by presburger
-  from d1 d2 have "(r, [], \<beta>'' @ \<beta>') \<leadsto>\<^sub>d (s, [], \<zeta>)" by simp
-  then have **: "\<exists>Z \<beta>'''. \<beta>''@\<beta>' = Z#\<beta>'''"
-    using step\<^sub>1_det_step\<^sub>1[of r "[]" "\<beta>'' @ \<beta>'" s "[]" \<zeta>] step\<^sub>1_nonempty_stack[of r "[]" "\<beta>'' @ \<beta>'" s "[]" \<zeta>] by simp
-  from \<beta>_def * ** show ?case by auto                                                                                          
+  from * obtain n where p3: "(q, [], [X]) \<leadsto>(n) (r, [], \<beta>'' @ \<beta>')"
+    using stepn_steps[of q "[]" "[X]" r "[]" "\<beta>'' @ \<beta>'"] by presburger
+  from assms(1) obtain s \<zeta> where p4: "(q, [], [X]) \<leadsto>(Suc n) (s, [], \<zeta>)" by presburger
+  from p4 have **: "(r, [], \<beta>'' @ \<beta>') \<leadsto> (s, [], \<zeta>)"
+    using stepn_split_last[of n q "[]" "[X]" s "[]" \<zeta>] dpda_stepn_det[OF p3] by auto
+  from \<beta>_def * show ?case 
+    using step\<^sub>1_nonempty_stack[OF **] by auto                                                                                    
 qed                                 
                                                                      
-text \<open>The automaton @{const scan_dpda} can either mimic the steps of the original automaton or detect a cycle\<close>
+text \<open>The automaton @{const [source] scan_dpda} can either mimic the steps of the original automaton or detect a cycle:\<close>
 lemma scan_dpda_steps:
   assumes "(q, w, \<alpha>) \<leadsto>* (p, u, \<gamma>)"
   shows "(OST q, w, map OSYM \<alpha>) \<leadsto>\<^sub>s* (OST p, u, map OSYM \<gamma>) \<or>     
-            (\<exists>r X \<beta>. (OST q, w, map OSYM \<alpha>) \<leadsto>\<^sub>s* (OST r, u, OSYM X # map OSYM \<beta>) \<and> (r, [], X#\<beta>) \<leadsto>* (p, [], \<gamma>) \<and> (\<forall>i. \<exists>s \<Delta>. (r, [], [X]) \<leadsto>\<^sub>d(i) (s, [], \<Delta>)))"
+            (\<exists>r X \<beta>. (OST q, w, map OSYM \<alpha>) \<leadsto>\<^sub>s* (OST r, u, OSYM X # map OSYM \<beta>) \<and> (r, [], X#\<beta>) \<leadsto>* (p, [], \<gamma>) \<and> (\<forall>i. \<exists>s \<Delta>. (r, [], [X]) \<leadsto>(i) (s, [], \<Delta>)))"
 using assms proof (induction "(q, w, \<alpha>)" "(p, u, \<gamma>)" arbitrary: p u \<gamma> rule: steps_induct2_bw)
   case base
   then show ?case
@@ -335,11 +474,11 @@ next
     case a    
     then obtain \<zeta> where v_def: "u = v" and \<beta>_def: "\<beta> = \<zeta> @ \<gamma>'" and elem: "(r, \<zeta>) \<in> \<delta>\<epsilon> M p X" by blast 
     from step(3) consider (a1) "(OST q, w, map OSYM \<alpha>) \<leadsto>\<^sub>s* (OST p, u, map OSYM \<gamma>)" |  
-                          (a2) "\<exists>r X \<beta>. (OST q, w, map OSYM \<alpha>) \<leadsto>\<^sub>s* (OST r, u, OSYM X # map OSYM \<beta>) \<and> (r, [], X # \<beta>) \<leadsto>* (p, [], \<gamma>) \<and> (\<forall>i. \<exists>s \<Delta>. (r, [], [X]) \<leadsto>\<^sub>d(i) (s, [], \<Delta>))" by blast
+                          (a2) "\<exists>r X \<beta>. (OST q, w, map OSYM \<alpha>) \<leadsto>\<^sub>s* (OST r, u, OSYM X # map OSYM \<beta>) \<and> (r, [], X # \<beta>) \<leadsto>* (p, [], \<gamma>) \<and> (\<forall>i. \<exists>s \<Delta>. (r, [], [X]) \<leadsto>(i) (s, [], \<Delta>))" by blast
     then show ?thesis
     proof cases    
-      case a1     
-      consider (a11) "\<forall>i. \<exists>s \<Delta>. (p, [], [X]) \<leadsto>\<^sub>d(i) (s, [], \<Delta>)" | (a12) "\<not>(\<forall>i. \<exists>s \<Delta>. (p, [], [X]) \<leadsto>\<^sub>d(i) (s, [], \<Delta>))" by blast
+      case a1   
+      consider (a11) "\<forall>i. \<exists>s \<Delta>. (p, [], [X]) \<leadsto>(i) (s, [], \<Delta>)" | (a12) "\<not>(\<forall>i. \<exists>s \<Delta>. (p, [], [X]) \<leadsto>(i) (s, [], \<Delta>))" by blast
       then show ?thesis
       proof cases
         case a11     
@@ -353,49 +492,47 @@ next
           by (auto simp: eps_nonfinal_def eps_final_def)
         with elem have "(OST r, map OSYM \<zeta>) \<in> \<delta>\<epsilon> scan_dpda (OST p) (OSYM X)"
           by (auto simp: scan_dpda_def)
-        with v_def \<gamma>_def \<beta>_def have "(OST p, u, map OSYM \<gamma>) \<leadsto>\<^sub>s (OST r, v, map OSYM \<beta>)"
+        with v_def \<gamma>_def \<beta>_def have *: "(OST p, u, map OSYM \<gamma>) \<leadsto>\<^sub>s (OST r, v, map OSYM \<beta>)"
           using scan.step\<^sub>1_rule[of "OST p" u "OSYM X" "map OSYM \<gamma>'" "OST r" u "map OSYM \<zeta> @ map OSYM \<gamma>'"] by simp
-        with a1 show ?thesis     
-          using scan.step\<^sub>1_steps scan.steps_trans by blast  
+        show ?thesis
+          using scan.steps_trans[OF a1 scan.step\<^sub>1_steps[OF *]] by satx  
       qed               
     next                                               
-      case a2                        
+      case a2         
       then obtain s Y \<mu> where *: "(OST q, w, map OSYM \<alpha>) \<leadsto>\<^sub>s* (OST s, u, OSYM Y # map OSYM \<mu>)" and spath: "(s, [], Y # \<mu>) \<leadsto>* (p, [], \<gamma>)"
-                          and **: "\<forall>i. \<exists>t \<Delta>. (s, [], [Y]) \<leadsto>\<^sub>d(i) (t, [], \<Delta>)" by blast 
-      from elem \<gamma>_def \<beta>_def have "(p, [], \<gamma>) \<leadsto> (r, [], \<beta>)"   
+                          and **: "\<forall>i. \<exists>t \<Delta>. (s, [], [Y]) \<leadsto>(i) (t, [], \<Delta>)" by blast 
+      from elem \<gamma>_def \<beta>_def have ***:"(p, [], \<gamma>) \<leadsto> (r, [], \<beta>)"   
         using step\<^sub>1_rule[of p "[]" X \<gamma>' r "[]" \<beta>] by simp  
-      with spath have ***: "(s, [], Y # \<mu>) \<leadsto>* (r, [], \<beta>)"
-        using step\<^sub>1_steps steps_trans by blast
-      from *[unfolded v_def] ** *** show ?thesis by blast           
+      have ****: "(s, [], Y # \<mu>) \<leadsto>* (r, [], \<beta>)"
+        using steps_trans[OF spath step\<^sub>1_steps[OF ***]] .
+      from *[unfolded v_def] ** **** show ?thesis by blast           
     qed                               
   next    
-    (* This is the only place we use determinism. *)
     case b  
     then obtain a \<zeta> where u_def: "u = a#v" and \<beta>_def: "\<beta> = \<zeta> @ \<gamma>'" and elem: "(r, \<zeta>) \<in> \<delta> M p a X" by blast
     from elem have eps_empty: "\<delta>\<epsilon> M p X = {}"               
       using \<delta>_nonempty[of p a X] by blast
     from step(3) consider (t) "(OST q, w, map OSYM \<alpha>) \<leadsto>\<^sub>s* (OST p, u, map OSYM \<gamma>)" 
-      | (f) "\<exists>r X \<beta>. (OST q, w, map OSYM \<alpha>) \<leadsto>\<^sub>s* (OST r, u, OSYM X # map OSYM \<beta>) \<and> (r, [], X # \<beta>) \<leadsto>* (p, [], \<gamma>) \<and> (\<forall>i. \<exists>s \<Delta>. (r, [], [X]) \<leadsto>\<^sub>d(i) (s, [], \<Delta>))" by blast
+      | (f) "\<exists>r X \<beta>. (OST q, w, map OSYM \<alpha>) \<leadsto>\<^sub>s* (OST r, u, OSYM X # map OSYM \<beta>) \<and> (r, [], X # \<beta>) \<leadsto>* (p, [], \<gamma>) \<and> (\<forall>i. \<exists>s \<Delta>. (r, [], [X]) \<leadsto>(i) (s, [], \<Delta>))" by blast
     then have *: "(OST q, w, map OSYM \<alpha>) \<leadsto>\<^sub>s* (OST p, u, map OSYM \<gamma>)"         
     proof cases
       case t
       then show ?thesis .
     next
-      case f     
-      then obtain s Y \<mu> where f1: "(s, [], Y # \<mu>) \<leadsto>* (p, [], \<gamma>)" and f2: "\<forall>i. \<exists>s' \<mu>'. (s, [], [Y]) \<leadsto>\<^sub>d(i) (s', [], \<mu>')" by blast 
+      case f
+      then obtain s Y \<mu> where f1: "(s, [], Y # \<mu>) \<leadsto>* (p, [], \<gamma>)" and f2: "\<forall>i. \<exists>s' \<mu>'. (s, [], [Y]) \<leadsto>(i) (s', [], \<mu>')" by blast 
       with \<gamma>_def obtain \<gamma>'' where "(s, [], [Y]) \<leadsto>* (p, [], X#\<gamma>'')"  
         using stack_cycle_drop[OF f2 f1] by blast 
-      then obtain n where f3: "(s, [], [Y]) \<leadsto>\<^sub>d(n) (p, [], X#\<gamma>'')"
-        using stepn_steps[of s "[]" "[Y]" p "[]" "X#\<gamma>''"] stepn_det_stepn\<^sub>1[of _ s "[]" "[Y]" p "[]" "X#\<gamma>''"] by blast  
-      from eps_empty have f4: "(p, [], X#\<gamma>'') \<leadsto>\<^sub>d" 
-        by (simp add: det_step_def the_elem_opt_def) 
-      from f3 f4 have "(s, [], [Y]) \<leadsto>\<^sub>d(Suc n)" by simp
+      then obtain n where f3: "(s, [], [Y]) \<leadsto>(n) (p, [], X#\<gamma>'')"
+        using stepn_steps[of s "[]" "[Y]" p "[]" "X#\<gamma>''"] by presburger 
+      from eps_empty have f4: "(p, [], X#\<gamma>'') \<leadsto>" by simp
+      from f4 have "(s, [], [Y]) \<leadsto>(Suc n)"
+        using stepn_split_last[of n s "[]" "[Y]"] dpda_stepn_det[OF f3] by fastforce
       with f2 have False
         using not_None_eq by blast
       then show ?thesis by simp            
     qed     
-    from eps_empty have "(p, [], [X]) \<leadsto>\<^sub>d(1)"
-      by (simp add: det_step_def the_elem_opt_def) 
+    from eps_empty have "(p, [], [X]) \<leadsto>(1)" by auto
     then have "\<not>eps_nonfinal p X \<and> \<not>eps_final p X"   
       unfolding eps_nonfinal_def eps_final_def using not_None_eq by blast
     with elem have "(OST r, map OSYM \<zeta>) \<in> \<delta> scan_dpda (OST p) a (OSYM X)" 
@@ -407,8 +544,9 @@ next
   qed                           
 qed
 
-text \<open>The language of @{const scan_dpda} and the original pushdown automaton are the same.\<close>
-lemma "scan.accept_final = accept_final"
+text \<open>The language of the automaton @{const [source] scan_dpda} and of the original automaton are the same, i.e. they are equivalent:\<close>
+lemma lang_scan_dpda:
+"scan.accept_final = accept_final"
 proof
   show "scan.accept_final \<subseteq> accept_final"
   proof
@@ -448,9 +586,9 @@ proof
         using scan_dpda_stepsX0[of "init_state M" w "[init_symbol M]" p' "[]" \<alpha>''] by simp
       from \<alpha>_def \<alpha>_with_X0 X_def obtain \<alpha>''' where \<alpha>''_def: "\<alpha>'' = X'#\<alpha>'''"
         by (metis Nil_is_map_conv append_Cons append_Nil hd_Cons_tl list.map_sel(1) list.sel(1) sym_extended.distinct(1) sym_extended.inject)
-      from epath[unfolded eps_final_def] obtain i r \<beta> where dpath: "(p', [], [X']) \<leadsto>\<^sub>d(i) (r, [], \<beta>)" and r_final: "r \<in> final_states M" by blast
-      from dpath have "(p', [], [X']) \<leadsto>* (r, [], \<beta>)"
-        using stepn_det_stepn\<^sub>1[of i p' "[]" "[X']" r "[]" \<beta>] stepn_steps[of p' "[]" "[X']" r "[]" \<beta>] by auto
+      from epath[unfolded eps_final_def] obtain i r \<beta> where path: "(p', [], [X']) \<leadsto>(i) (r, [], \<beta>)" and r_final: "r \<in> final_states M" by blast
+      from path have "(p', [], [X']) \<leadsto>* (r, [], \<beta>)"
+        using stepn_steps[of p' "[]" "[X']" r "[]" \<beta>] by auto
       with \<alpha>''_def have **: "(p', [], \<alpha>'') \<leadsto>* (r, [], \<beta>@\<alpha>''')"
         using steps_stack_app[of p' "[]" "[X']" r "[]" \<beta> \<alpha>'''] by simp
       from r_final show ?thesis
@@ -468,7 +606,7 @@ next
       using scan_dpda_def scan.step\<^sub>1_rule by auto
     from scan_dpda_steps[OF p] consider (a) "(OST (init_state M), w, [OSYM (init_symbol M)]) \<leadsto>\<^sub>s* (OST q, [], map OSYM \<gamma>)"
       | (b) "\<exists>r X \<beta>. (OST (init_state M), w, [OSYM (init_symbol M)]) \<leadsto>\<^sub>s* (OST r, [], OSYM X # map OSYM \<beta>) \<and>
-                                (r, [], X # \<beta>) \<leadsto>* (q, [], \<gamma>) \<and> (\<forall>i. \<exists>s \<Delta>. (r, [], [X]) \<leadsto>\<^sub>d(i) (s, [], \<Delta>))" by auto
+                                (r, [], X # \<beta>) \<leadsto>* (q, [], \<gamma>) \<and> (\<forall>i. \<exists>s \<Delta>. (r, [], [X]) \<leadsto>(i) (s, [], \<Delta>))" by auto
     then show "w \<in> scan.accept_final"
     proof cases
       case a
@@ -481,15 +619,15 @@ next
     next
       case b
       then obtain r X \<beta> where pscan: "(OST (init_state M), w, [OSYM (init_symbol M)]) \<leadsto>\<^sub>s* (OST r, [], OSYM X # map OSYM \<beta>)" and
-        pr: "(r, [], X # \<beta>) \<leadsto>* (q, [], \<gamma>)" and cycle: "\<forall>i. \<exists>s \<Delta>. (r, [], [X]) \<leadsto>\<^sub>d(i) (s, [], \<Delta>)" by blast
+        pr: "(r, [], X # \<beta>) \<leadsto>* (q, [], \<gamma>)" and cycle: "\<forall>i. \<exists>s \<Delta>. (r, [], [X]) \<leadsto>(i) (s, [], \<Delta>)" by blast
       have *: "(OST (init_state M), w, [OSYM (init_symbol M), X0]) \<leadsto>\<^sub>s* (OST r, [], stack_with_X0 (X # \<beta>))"
         using scan.steps_stack_app[OF pscan] by simp
       have r_final: "\<exists>\<gamma>'. (r, [], [X]) \<leadsto>* (q, [], \<gamma>')"
         using stack_cycle_drop[OF cycle pr] by auto
       from r_final q_final have e1: "\<not>eps_nonfinal r X"
-        unfolding eps_nonfinal_def using stepn_steps[of r "[]" "[X]" q "[]"] stepn_det_stepn\<^sub>1[of _ r "[]" "[X]" q "[]"] by (metis option.inject prod.inject)
+        unfolding eps_nonfinal_def using stepn_steps[of r "[]" "[X]" q "[]"] dpda_stepn_det[of _ r "[]" "[X]" q "[]"] by blast
       from cycle r_final q_final have e2: "eps_final r X"
-        unfolding eps_final_def using stepn_steps[of r "[]" "[X]" q "[]"] stepn_det_stepn\<^sub>1[of _ r "[]" "[X]" q "[]"] by blast
+        unfolding eps_final_def using stepn_steps[of r "[]" "[X]" q "[]"] by blast
       from e1 e2 have "(OST r, [], OSYM X # map OSYM \<beta>) \<leadsto>\<^sub>s (F, [], OSYM X # map OSYM \<beta>)"
         using scan_dpda_def scan.step\<^sub>1_rule[of "OST r" "[]" "OSYM X" "map OSYM \<beta>" F "[]" "OSYM X # map OSYM \<beta>"] by simp
       then have **: "(OST r, [], stack_with_X0 (X#\<beta>)) \<leadsto>\<^sub>s (F, [], stack_with_X0 (X#\<beta>))"
@@ -501,11 +639,340 @@ next
     qed
   qed                                               
 qed
-                                                            
-(* TODO: Properties of scan_dpda *)
+
+subsubsection \<open>Scan Property\<close>
+
+lemma D_consumes: "(D, w, X#\<alpha>) \<leadsto>\<^sub>s* (D, [], X#\<alpha>)"
+proof (induction w)
+  case Nil
+  then show ?case
+    by (simp add: scan.steps_refl)
+next
+  case (Cons a w)
+  have "(D, [X]) \<in> scan_dpda_delta D a X" by simp
+  then have *: "(D, a#w, X#\<alpha>) \<leadsto>\<^sub>s (D, w, X#\<alpha>)"
+    using scan.step\<^sub>1_rule[of D "a#w" X \<alpha> D w "X#\<alpha>"] by (simp add: scan_dpda_def)
+  show ?case
+    using scan.steps_trans[OF scan.step\<^sub>1_steps[OF *] Cons] .
+qed
+
+definition eps_inf :: "'q \<Rightarrow> 's \<Rightarrow> bool" where
+  "eps_inf q X \<equiv> \<forall>i. \<exists>p \<alpha>. (q, [], [X]) \<leadsto>(i) (p, [], \<alpha>)"
+
+definition eps_infl :: "'q \<Rightarrow> 's list \<Rightarrow> bool" where
+  "eps_infl q \<alpha> \<equiv> \<forall>i. \<exists>p \<gamma>. (q, [], \<alpha>) \<leadsto>(i) (p, [], \<gamma>)"
+
+text \<open>If a pair of a state and a stack symbol does not allow infinite epsilon steps, then the stack symbol will be consumed:\<close>
+lemma inf_consumes_sym:
+  assumes "eps_infl q (X#\<alpha>)"
+      and "\<not>eps_inf q X"
+    shows "\<exists>p. (q, [], X#\<alpha>) \<leadsto>* (p, [], \<alpha>)"
+proof (rule ccontr)
+  assume asm: "\<nexists>p. (q, [], X#\<alpha>) \<leadsto>* (p, [], \<alpha>)"
+  have "\<exists>p \<gamma>. (q, [], X#\<alpha>) \<leadsto>(i) (p, [], \<gamma>@\<alpha>) \<and> \<gamma> \<noteq> [] \<and> (q, [], [X]) \<leadsto>(i) (p, [], \<gamma>)" for i
+  proof (induct i)
+    case 0
+    have "(q, [], X # \<alpha>) \<leadsto>(0) (q, [], [X] @ \<alpha>) \<and> [X] \<noteq> [] \<and> (q, [], [X]) \<leadsto>(0) (q, [], [X])" by simp
+    then show ?case by metis
+  next
+    case (Suc i)
+    then obtain p \<gamma> where p: "(q, [], X # \<alpha>) \<leadsto>(i) (p, [], \<gamma> @ \<alpha>)" and \<gamma>_def: "\<gamma> \<noteq> []" and p1: "(q, [], [X]) \<leadsto>(i) (p, [], \<gamma>)" by blast
+    from assms(1)[unfolded eps_infl_def] obtain r \<beta> where *: "(q, [], X#\<alpha>) \<leadsto>(Suc i) (r, [], \<beta>)" by blast
+    then have st: "(p, [], \<gamma>@\<alpha>) \<leadsto> (r, [], \<beta>)"
+      using stepn_split_last[of i q "[]" "X#\<alpha>" r "[]" \<beta>] dpda_stepn_det[OF p] by auto
+    from \<gamma>_def obtain Y \<gamma>' where \<gamma>_def2: "\<gamma> = Y#\<gamma>'"
+      using list.exhaust by blast
+    from st[unfolded \<gamma>_def2] obtain \<gamma>'' where \<beta>_def: "\<beta> = \<gamma>'' @ \<gamma>' @ \<alpha>"
+      using step\<^sub>1_rule[of p "[]" Y "\<gamma>'@\<alpha>" r "[]" \<beta>] by auto
+    from *[unfolded \<beta>_def] asm have **: "\<gamma>'' @ \<gamma>' \<noteq> []"
+      using stepn_steps[of q "[]" "X#\<alpha>" r "[]" "\<gamma>'' @ \<gamma>' @ \<alpha>"] by force
+    from st[unfolded \<beta>_def] \<gamma>_def have st1: "(p, [], \<gamma>) \<leadsto> (r, [], \<gamma>'' @ \<gamma>')"
+      using step\<^sub>1_stack_drop[of p "[]" \<gamma> \<alpha> r "[]" "\<gamma>'' @ \<gamma>'"] by simp
+    from p1 st1 have ***: "(q, [], [X]) \<leadsto>(Suc i) (r, [], \<gamma>'' @ \<gamma>')" by simp
+    from *[unfolded \<beta>_def] ** *** show ?case
+      by (metis append.assoc)
+  qed
+  then have "eps_inf q X"
+    by (metis eps_inf_def)
+  with assms(2) show False by satx
+qed
+
+lemma some_pair_inf:
+  assumes "eps_infl q \<alpha>"
+      and "\<And>p X \<gamma>. (q, [], \<alpha>) \<leadsto>* (p, [], X#\<gamma>) \<longrightarrow> \<not>eps_inf p X"
+    shows False
+using assms proof (induction \<alpha> arbitrary: q)
+  case Nil
+  then show ?case
+    by (force simp: eps_infl_def)
+next
+  case (Cons X \<alpha>)
+  from Cons(3)[of q X \<alpha>] have e: "\<not>eps_inf q X"
+    by (simp add: steps_refl)
+  obtain p where p: "(q, [], X#\<alpha>) \<leadsto>* (p, [], \<alpha>)"
+    using inf_consumes_sym[OF Cons(2) e] by blast
+  then obtain i where p1: "(q, [], X#\<alpha>) \<leadsto>(i) (p, [], \<alpha>)"
+    using stepn_steps[of q "[]" "X#\<alpha>" p "[]" \<alpha>] by blast
+  have *: "eps_infl p \<alpha>" unfolding eps_infl_def proof
+    fix j
+    from Cons(2)[unfolded eps_infl_def] obtain r \<beta> where p2: "(q, [], X#\<alpha>) \<leadsto>(i + j) (r, [], \<beta>)" by blast
+    have "(p, [], \<alpha>) \<leadsto>(j) (r, [], \<beta>)"
+      using split_path[OF p2, of i] dpda_stepn_det[OF p1] by auto
+    then show "\<exists>r \<beta>. (p, [], \<alpha>) \<leadsto>(j) (r, [], \<beta>)" by blast
+  qed
+  from Cons(3) have **: "\<And>r Y \<gamma>. (p, [], \<alpha>) \<leadsto>* (r, [], Y # \<gamma>) \<longrightarrow> \<not> eps_inf r Y"
+    using steps_trans[OF p] by blast
+  from Cons(1)[OF * **] show ?case .
+qed
+
+text \<open>If a configuration allows infinite epsilon steps, it will eventually reach a pair of a 
+      state and a stack symbol that allows infinite epsilon steps:\<close>
+lemma inf_reaches:
+  assumes "eps_infl q \<alpha>"
+  shows "\<exists>p X \<gamma>. (q, [], \<alpha>) \<leadsto>* (p, [], X#\<gamma>) \<and> eps_inf p X"
+using assms some_pair_inf by blast
+
+lemma eps_inf_to_D:
+  assumes "eps_inf q X"
+  shows "(OST q, w, OSYM X # \<alpha>) \<leadsto>\<^sub>s* (D, [], OSYM X # \<alpha>)"
+proof -
+  from assms consider (a) "eps_nonfinal q X" | (b) "\<not>eps_nonfinal q X \<and> eps_final q X"
+    unfolding eps_inf_def eps_nonfinal_def eps_final_def by blast
+  then show ?thesis proof cases
+    case a
+    then have "(D, [OSYM X]) \<in> scan_dpda_delta_eps (OST q) (OSYM X)" by simp
+    then have st: "(OST q, w, OSYM X # \<alpha>) \<leadsto>\<^sub>s (D, w, OSYM X # \<alpha>)"
+      using scan.step\<^sub>1_rule[of "OST q" w "OSYM X" \<alpha> D w "OSYM X # \<alpha>"] by (simp add: scan_dpda_def)
+    show ?thesis
+      using scan.steps_trans[OF scan.step\<^sub>1_steps[OF st] D_consumes] .
+  next
+    case b
+    then have "(F, [OSYM X]) \<in> scan_dpda_delta_eps (OST q) (OSYM X)" by simp
+    then have st1: "(OST q, w, OSYM X # \<alpha>) \<leadsto>\<^sub>s (F, w, OSYM X # \<alpha>)"
+      using scan.step\<^sub>1_rule[of "OST q" w "OSYM X" \<alpha> F w "OSYM X # \<alpha>"] by (simp add: scan_dpda_def)
+    have "(D, [OSYM X]) \<in> scan_dpda_delta_eps F (OSYM X)" by simp
+    then have st2: "(F, w, OSYM X # \<alpha>) \<leadsto>\<^sub>s (D, w, OSYM X # \<alpha>)"
+      using scan.step\<^sub>1_rule[of F w  "OSYM X" \<alpha> D w "OSYM X # \<alpha>"] by (simp add: scan_dpda_def)
+    show ?thesis
+      using scan.steps_trans[OF scan.step\<^sub>1_steps[OF st1] scan.steps_trans[OF scan.step\<^sub>1_steps[OF st2] D_consumes]] .
+  qed
+qed
+
+lemma scan_dpda_eps_inf:
+  assumes "(q, w, \<alpha>) \<leadsto>* (p, w, X#\<gamma>)"
+      and "eps_inf p X"
+    shows "\<exists>Y \<beta>. (OST q, w, map OSYM \<alpha>) \<leadsto>\<^sub>s* (D, [], OSYM Y # \<beta>)"
+proof -
+  consider (a) "(OST q, w, map OSYM \<alpha>) \<leadsto>\<^sub>s* (OST p, w, OSYM X # map OSYM \<gamma>)" |
+           (b) "\<exists>r Y \<beta>. (OST q, w, map OSYM \<alpha>) \<leadsto>\<^sub>s* (OST r, w, OSYM Y # map OSYM \<beta>) \<and> (\<forall>i. \<exists>s \<zeta>. (r, [], [Y]) \<leadsto>(i) (s, [], \<zeta>))"
+    using scan_dpda_steps[OF assms(1)] by auto
+  then show ?thesis proof cases
+    case a
+    have *: "(OST p, w, OSYM X # map OSYM \<gamma>) \<leadsto>\<^sub>s* (D, [], OSYM X # map OSYM \<gamma>)"
+      using eps_inf_to_D[OF assms(2)] by simp
+    show ?thesis
+      using scan.steps_trans[OF a *] by blast
+  next
+    case b
+    then obtain r Y \<beta> where p: "(OST q, w, map OSYM \<alpha>) \<leadsto>\<^sub>s* (OST r, w, OSYM Y # map OSYM \<beta>)" and r_inf: "\<forall>i. \<exists>s \<zeta>. (r, [], [Y]) \<leadsto>(i) (s, [], \<zeta>)" by blast
+    from r_inf have r_eps_inf: "eps_inf r Y"
+      by (simp add: eps_inf_def)
+    have *: "(OST r, w, OSYM Y # map OSYM \<beta>) \<leadsto>\<^sub>s* (D, [], OSYM Y # map OSYM \<beta>)"
+      using eps_inf_to_D[OF r_eps_inf] by simp
+    show ?thesis
+      using scan.steps_trans[OF p *] by blast
+  qed
+qed
+
+lemma scan_dpda_neps_infl:
+  assumes "\<not>eps_infl q \<alpha>"
+  shows "\<exists>p \<gamma>. (OST q, w, map OSYM \<alpha>) \<leadsto>\<^sub>s* (OST p, w, map OSYM \<gamma>) \<and> (\<forall>X \<gamma>'. \<gamma> = X#\<gamma>' \<longrightarrow> \<delta>\<epsilon> M p X = {})"
+proof -
+  from assms[unfolded eps_infl_def] obtain i where "\<forall>p \<gamma>. \<not>(q, [], \<alpha>) \<leadsto>(i) (p, [], \<gamma>)" by blast
+  then have "\<exists>j p \<gamma>. j < i \<and> (q, [], \<alpha>) \<leadsto>(j) (p, [], \<gamma>) \<and> (p, [], \<gamma>) \<leadsto>" proof (induction i)
+    case 0
+    then show ?case
+      by (auto simp: steps_refl)
+  next
+    case (Suc i)
+    consider (a) "\<forall>p \<gamma>. \<not> (q, [], \<alpha>) \<leadsto>(i) (p, [], \<gamma>)" | (b) "\<exists>p \<gamma>. (q, [], \<alpha>) \<leadsto>(i) (p, [], \<gamma>)" by blast
+    then show ?case proof cases
+      case a
+      from Suc(1)[OF a] show ?thesis
+        by (auto simp: less_Suc_eq)
+    next
+      case b
+      then obtain p \<gamma> where *: "(q, [], \<alpha>) \<leadsto>(i) (p, [], \<gamma>)" by blast
+      with Suc(2) have **: "(p, [], \<gamma>) \<leadsto>"
+        using decreasing_word step\<^sub>1_steps by fastforce
+      from * ** show ?thesis by blast
+    qed
+  qed
+  then obtain j p \<gamma> where "j < i" and p: "(q, [], \<alpha>) \<leadsto>(j) (p, [], \<gamma>)" and nst: "(p, [], \<gamma>) \<leadsto>" by blast
+  from p have p1: "(q, [], \<alpha>) \<leadsto>* (p, [], \<gamma>)"
+    using stepn_steps[of q "[]" \<alpha> p "[]" \<gamma>] by auto
+  consider (a) "(OST q, [], map OSYM \<alpha>) \<leadsto>\<^sub>s* (OST p, [], map OSYM \<gamma>)" |
+           (b) "\<exists>r X \<beta>. (OST q, [], map OSYM \<alpha>) \<leadsto>\<^sub>s* (OST r, [], OSYM X # map OSYM \<beta>) \<and> (\<forall>i. \<exists>s \<Delta>. (r, [], [X]) \<leadsto>(i) (s, [], \<Delta>))"
+    using scan_dpda_steps[OF p1] by blast
+  then show ?thesis proof cases
+    case a
+    then have *: "(OST q, w, map OSYM \<alpha>) \<leadsto>\<^sub>s* (OST p, w, map OSYM \<gamma>)"
+      using scan.steps_word_app[of "OST q" "[]" "map OSYM \<alpha>" "OST p" "[]" "map OSYM \<gamma>" w] by simp
+    from nst have **: "\<forall>X \<gamma>'. \<gamma> = X # \<gamma>' \<longrightarrow> \<delta>\<epsilon> M p X = {}" by auto
+    from * ** show ?thesis by blast
+  next
+    case b
+    then obtain r X \<beta> where p2: "(OST q, [], map OSYM \<alpha>) \<leadsto>\<^sub>s* (OST r, [], OSYM X # map OSYM \<beta>)" and cycle: "\<forall>i. \<exists>s \<Delta>. (r, [], [X]) \<leadsto>(i) (s, [], \<Delta>)" by blast
+    from p2 have p3: "(OST q, [], stack_with_X0 \<alpha>) \<leadsto>\<^sub>s* (OST r, [], stack_with_X0 (X#\<beta>))"
+      using scan.steps_stack_app[where ?\<beta> = "[X0]"] by fastforce
+    have "(q, [], \<alpha>) \<leadsto>* (r, [], X#\<beta>)"
+      using scan_dpda_stepsX0[OF p3] .
+    then obtain n where p4: "(q, [], \<alpha>) \<leadsto>(n) (r, [], X#\<beta>)"
+      using stepn_steps[of q "[]" \<alpha> r "[]" "X#\<beta>"] by blast
+    have "\<forall>k. \<exists>s \<Delta>. (q, [], \<alpha>) \<leadsto>(k) (s, [], \<Delta>)" proof
+      fix k
+      show "\<exists>s \<Delta>. (q, [], \<alpha>) \<leadsto>(k) (s, [], \<Delta>)" proof (cases "k < n")
+        case True
+        then have k_leq: "k \<le> n" by simp
+        then obtain s u \<zeta> where *: "(q, [], \<alpha>) \<leadsto>(k) (s, u, \<zeta>)"
+          using split_path[OF p4 k_leq] by blast
+        from * have u_def: "u = []"
+          using stepn_steps[of q "[]" \<alpha> s u \<zeta>] decreasing_word[of q "[]" \<alpha> s u \<zeta>] by auto
+        from *[unfolded u_def] show ?thesis by blast
+      next
+        case False
+        then have k_beq: "k \<ge> n" by simp
+        with cycle obtain s \<zeta> where "(r, [], [X]) \<leadsto>(k-n) (s, [], \<zeta>)" by presburger
+        then have p5: "(r, [], X#\<beta>) \<leadsto>(k-n) (s, [], \<zeta>@\<beta>)"
+          using stepn_stack_app[where ?\<beta> = \<beta>] by fastforce
+        from k_beq show ?thesis
+          using stepn_trans[OF p4 p5] by auto 
+      qed
+    qed
+    with assms show ?thesis
+      by (simp add: eps_infl_def)
+  qed
+qed
+
+lemma scan_dpda_scans_OST:
+"\<exists>p X \<gamma>. (OST q, w, stack_with_X0 \<alpha>) \<leadsto>\<^sub>s* (p, [], X#\<gamma>) \<and> \<delta> scan_dpda p a X \<noteq> {}"
+proof (induction w arbitrary: q \<alpha>)
+  case Nil
+  then show ?case proof (cases "eps_infl q \<alpha>")
+    case True
+    obtain p X \<gamma> where p: "(q, [], \<alpha>) \<leadsto>* (p, [], X#\<gamma>)" and eps_p: "eps_inf p X"
+      using inf_reaches[OF True] by blast
+    obtain Y \<beta> where "(OST q, [], map OSYM \<alpha>) \<leadsto>\<^sub>s* (D, [], OSYM Y # \<beta>)"
+      using scan_dpda_eps_inf[OF p eps_p] by blast
+    then have *: "(OST q, [], stack_with_X0 \<alpha>) \<leadsto>\<^sub>s* (D, [], OSYM Y # \<beta> @ [X0])"
+      using scan.steps_stack_app[where ?\<beta> = "[X0]"] by fastforce
+    have **: "\<delta> scan_dpda D a (OSYM Y) \<noteq> {}"
+      by (simp add: scan_dpda_def)
+    from * ** show ?thesis by blast
+  next
+    case False
+    obtain p \<gamma> where p: "(OST q, [], map OSYM \<alpha>) \<leadsto>\<^sub>s* (OST p, [], map OSYM \<gamma>)" and \<gamma>_nempty: "(\<forall>X \<gamma>'. \<gamma> = X#\<gamma>' \<longrightarrow> \<delta>\<epsilon> M p X = {})"
+      using scan_dpda_neps_infl[OF False] by blast
+    from p have p1: "(OST q, [], stack_with_X0 \<alpha>) \<leadsto>\<^sub>s* (OST p, [], stack_with_X0 \<gamma>)"
+      using scan.steps_stack_app[where ?\<beta> = "[X0]"] by simp
+    show ?thesis proof (cases \<gamma>)
+      case Nil
+      with p1 show ?thesis
+        by (force simp: scan_dpda_def)
+    next
+      case (Cons X \<gamma>')
+      with \<gamma>_nempty have "\<delta>\<epsilon> M p X = {}" by simp
+      then have "\<delta> scan_dpda (OST p) a (OSYM X) \<noteq> {}"
+        by (simp add: scan_dpda_def)
+      with p1 Cons show ?thesis by auto
+    qed
+  qed
+next
+  case IH: (Cons b w)
+  show ?case proof (cases "eps_infl q \<alpha>")
+    case True
+    obtain p X \<gamma> where p: "(q, [], \<alpha>) \<leadsto>* (p, [], X#\<gamma>)" and eps_p: "eps_inf p X"
+      using inf_reaches[OF True] by blast
+    from p have p1: "(q, b#w, \<alpha>) \<leadsto>* (p, b#w, X#\<gamma>)"
+      using steps_word_app[of q "[]" \<alpha> p "[]" "X#\<gamma>" "b#w"] by simp
+    obtain Y \<beta> where "(OST q, b # w, map OSYM \<alpha>) \<leadsto>\<^sub>s* (D, [], OSYM Y # \<beta>)"
+      using scan_dpda_eps_inf[OF p1 eps_p] by blast
+    then have *: "(OST q, b # w, stack_with_X0 \<alpha>) \<leadsto>\<^sub>s* (D, [], OSYM Y # \<beta> @ [X0])"
+      using scan.steps_stack_app[where ?\<beta> = "[X0]"] by fastforce
+    have **: "\<delta> scan_dpda D a (OSYM Y) \<noteq> {}"
+      by (simp add: scan_dpda_def)
+    from * ** show ?thesis by blast
+  next
+    case False
+    obtain p \<gamma> where p: "(OST q, b#w, map OSYM \<alpha>) \<leadsto>\<^sub>s* (OST p, b#w, map OSYM \<gamma>)" and \<gamma>_nempty: "(\<forall>X \<gamma>'. \<gamma> = X#\<gamma>' \<longrightarrow> \<delta>\<epsilon> M p X = {})"
+      using scan_dpda_neps_infl[OF False] by blast
+    from p have p1: "(OST q, b#w, stack_with_X0 \<alpha>) \<leadsto>\<^sub>s* (OST p, b#w, stack_with_X0 \<gamma>)"
+      using scan.steps_stack_app[where ?\<beta> = "[X0]"] by simp
+    show ?thesis proof (cases \<gamma>)
+      case Nil
+      have "(D, [X0]) \<in> scan_dpda_delta (OST p) b X0" by simp
+      with Nil have st: "(OST p, b#w, stack_with_X0 \<gamma>) \<leadsto>\<^sub>s (D, w, [X0])"
+        using scan.step\<^sub>1_rule[of "OST p" "b#w" X0 "[]" D w "[X0]"] by (simp add: scan_dpda_def)
+      have *: "(OST q, b#w, stack_with_X0 \<alpha>) \<leadsto>\<^sub>s* (D, [], [X0])"
+        using scan.steps_trans[OF p1 scan.steps_trans[OF scan.step\<^sub>1_steps[OF st] D_consumes]] .
+      have **: "\<delta> scan_dpda D a X0 \<noteq> {}"
+        by (simp add: scan_dpda_def)
+      from * ** show ?thesis by blast
+    next
+      case (Cons X \<gamma>')
+      with \<gamma>_nempty have "\<delta>\<epsilon> M p X = {}" by simp
+      then consider (a) "(D, [OSYM X]) \<in> scan_dpda_delta (OST p) b (OSYM X)" | (b) "\<exists>r \<beta>. (OST r, map OSYM \<beta>) \<in> scan_dpda_delta (OST p) b (OSYM X)"
+        by (cases "\<delta> M p b X = {}") fastforce+
+      then show ?thesis proof cases
+        case a
+        with Cons have st: "(OST p, b#w, stack_with_X0 \<gamma>) \<leadsto>\<^sub>s (D, w, stack_with_X0 \<gamma>)"
+          using scan.step\<^sub>1_rule[of "OST p" "b#w" "OSYM X" "stack_with_X0 \<gamma>'" D w "stack_with_X0 \<gamma>"] by (simp add: scan_dpda_def)
+        from Cons have *: "(OST q, b#w, stack_with_X0 \<alpha>) \<leadsto>\<^sub>s* (D, [], stack_with_X0 \<gamma>)"
+          using scan.steps_trans[OF p1 scan.steps_trans[OF scan.step\<^sub>1_steps[OF st]]] D_consumes[of w "OSYM X" "stack_with_X0 \<gamma>'"] by simp
+        have **: "\<delta> scan_dpda D a (OSYM X) \<noteq> {}"
+          by (simp add: scan_dpda_def)
+        from * ** Cons show ?thesis by auto
+      next
+        case b
+        then obtain r \<beta> where "(OST r, map OSYM \<beta>) \<in> scan_dpda_delta (OST p) b (OSYM X)" by blast
+        with Cons have st: "(OST p, b#w, stack_with_X0 \<gamma>) \<leadsto>\<^sub>s (OST r, w, stack_with_X0 (\<beta>@\<gamma>'))"
+          using scan.step\<^sub>1_rule[of "OST p" "b#w" "OSYM X" "stack_with_X0 \<gamma>'" "OST r" w "stack_with_X0 (\<beta>@\<gamma>')"] by (simp add: scan_dpda_def)
+        from IH have *: "\<exists>p X \<gamma>. (OST r, w, stack_with_X0 (\<beta>@\<gamma>')) \<leadsto>\<^sub>s* (p, [], X # \<gamma>) \<and> \<delta> scan_dpda p a X \<noteq> {}" by presburger
+        from * show ?thesis
+          using scan.steps_trans[OF scan.steps_trans[OF p1 scan.step\<^sub>1_steps[OF st]]] by blast
+      qed
+    qed
+  qed
+qed
+
+text \<open>For every input word, the automaton @{const [source] scan_dpda} scans the entire input and, moreover, 
+      ends in a configuration where no epsilon step is possible:\<close>
+lemma scan_dpda_scans:
+"\<exists>q X \<alpha>. (init_state scan_dpda, w, [init_symbol scan_dpda]) \<leadsto>\<^sub>s* (q, [], X#\<alpha>) \<and> \<delta> scan_dpda q a X \<noteq> {}"
+proof -
+  have "(OST (init_state M), stack_with_X0 [init_symbol M]) \<in> scan_dpda_delta_eps Q0' X0" by simp
+  then have *: "(init_state scan_dpda, w, [init_symbol scan_dpda]) \<leadsto>\<^sub>s (OST (init_state M), w, stack_with_X0 [init_symbol M])"
+    using scan.step\<^sub>1_rule[of Q0' w X0 "[]" "OST (init_state M)" w "stack_with_X0 [init_symbol M]"] by (simp add: scan_dpda_def)
+  obtain p X \<gamma> where **: "(OST (init_state M), w, stack_with_X0 [init_symbol M]) \<leadsto>\<^sub>s* (p, [], X#\<gamma>)" and d: "\<delta> scan_dpda p a X \<noteq> {}"
+    using scan_dpda_scans_OST[of "init_state M" w "[init_symbol M]"] by blast
+  have "(init_state scan_dpda, w, [init_symbol scan_dpda]) \<leadsto>\<^sub>s* (p, [], X#\<gamma>)"
+    using scan.steps_trans[OF scan.step\<^sub>1_steps[OF *] **] .
+  with d show ?thesis by blast
+qed
 
 end
 
+subsection \<open>Complement Construction\<close>
+
+text \<open>After ensuring that the automaton scans its entire input word, we are left with constructing the deterministic 
+      pushdown automaton that recognizes the complement language. The main idea is to keep track of whether a final 
+      state has been visited since the last true step using a second component for states. If no final state has been 
+      visited, the complement automaton enters a final state of its own just before the next true step.\<close>
+
+subsubsection \<open>Definition\<close>
+
+text \<open>An S1-state indicates that a final state has been visited since the last true step, whereas an S2-state indicates 
+      that no final state has been visited since the last true step. S3-states are the final states of the complement automaton:\<close>
 datatype 'q st_num = S1 'q | S2 'q | S3 'q
 
 instance st_num :: (finite) finite
@@ -522,8 +989,9 @@ lemma inj_S1: "inj S1"
 lemma inj_S2: "inj S2"
   by (simp add: inj_def)
 
-locale complement_dpda = dpda M for M :: "('q :: finite, 'a :: finite, 's :: finite) pda"
-(* TODO: Assumptions about M *)
+text \<open>We can now assume the scan property proved in the last subsection:\<close>
+locale complement_dpda = dpda M for M :: "('q :: finite, 'a :: finite, 's :: finite) pda" +
+  assumes M_path: "\<exists>q X \<alpha>. (init_state M, w, [init_symbol M]) \<leadsto>* (q, [], X#\<alpha>) \<and> \<delta> M q a X \<noteq> {}"
 begin
 
 definition comp_dpda_init_state :: "'q st_num" where
@@ -547,12 +1015,14 @@ definition comp_dpda :: "('q st_num, 'a, 's) pda" where
   "comp_dpda \<equiv> \<lparr> init_state = comp_dpda_init_state, init_symbol = init_symbol M, final_states = comp_dpda_final_states,
                     delta = comp_dpda_delta, delta_eps = comp_dpda_delta_eps \<rparr>"
 
-(* TODO *)
+subsubsection \<open>Determinism\<close>
+
 lemma image_singleton_if_inj:
   assumes "inj f"
   shows "(\<exists>x. A = {x}) \<longleftrightarrow> (\<exists>x. f ` A = {x})"
 using assms by (metis image_empty image_insert image_inv_f_f)
 
+text \<open>The automaton @{const [source] comp_dpda} is deterministic:\<close>
 lemma dpda_comp_dpda: "dpda comp_dpda"
 proof (standard, goal_cases)
   case (1 p a Z)
@@ -624,30 +1094,412 @@ next
     by (simp add: comp_dpda_def)
 qed
 
+subsubsection \<open>Complementation\<close>
+
 sublocale comp: dpda comp_dpda
   using dpda_comp_dpda . 
 
-lemma h1: "w \<notin> accept_final \<Longrightarrow> w \<in> comp.accept_final"
-  sorry
+text \<open>We abbreviate the definitions of @{const [source] comp_dpda} with sub-index c:\<close>
+notation comp.step\<^sub>1 ("(_ \<leadsto>\<^sub>c _)" [50, 50] 50)
+notation comp.steps ("(_ \<leadsto>\<^sub>c* _)" [50, 50] 50)
+notation comp.nstep\<^sub>1 ("(_ \<leadsto>\<^sub>c)" [50] 50)
+notation comp.stepsn ("(_ /\<leadsto>\<^sub>c'(_')/ _)" [50, 0, 50] 50)
+notation comp.stepst ("(_ \<leadsto>\<^sub>c+ _)" [50, 50] 50)
 
-lemma h2: "w \<in> accept_final \<Longrightarrow> w \<notin> comp.accept_final"
-  sorry
+lemma comp_dpda_step_from_S1:
+  assumes "(S1 q, [], \<alpha>) \<leadsto>\<^sub>c (p, [], \<gamma>)"
+  shows "\<exists>p'. p = S1 p'"
+using assms comp.step\<^sub>1_rule_ext[of "S1 q" "[]" \<alpha> p "[]" \<gamma>] by (auto simp: comp_dpda_def)
 
-lemma h3: "w \<in> comp.accept_final \<Longrightarrow> w \<notin> accept_final"
-  sorry
+lemma comp_dpda_steps_from_S1:
+  assumes "(S1 q, [], \<alpha>) \<leadsto>\<^sub>c* (p, [], \<gamma>)"
+  shows "\<exists>p'. p = S1 p'"
+using assms comp_dpda_step_from_S1 comp.decreasing_word 
+  by (induction "(S1 q, [] :: 'a list, \<alpha>)" "(p, [] :: 'a list, \<gamma>)" arbitrary: p \<gamma> rule: comp.steps_induct2_bw) fastforce+
 
-lemma h4: "w \<notin> comp.accept_final \<Longrightarrow> w \<in> accept_final"
-  sorry
+lemma comp_dpda_nonfinal_stepsS2:
+  assumes "(q, [], \<alpha>) \<leadsto>* (p, [], \<gamma>)"
+      and "\<And>r \<beta>. (q, [], \<alpha>) \<leadsto>* (r, [], \<beta>) \<longrightarrow> r \<notin> final_states M"
+    shows "(S2 q, [], \<alpha>) \<leadsto>\<^sub>c* (S2 p, [], \<gamma>)"
+using assms proof (induction "(q, [] :: 'a list, \<alpha>)" "(p, [] :: 'a list, \<gamma>)" arbitrary: q \<alpha> rule: steps_induct2)
+  case 1
+  then show ?case
+    by (simp add: comp.steps_refl)
+next
+  case (2 q \<alpha> r u \<beta>)
+  from 2(1) obtain X \<alpha>' \<zeta> where \<alpha>_def: "\<alpha> = X#\<alpha>'" and u_def: "u = []" and *: "\<beta> = \<zeta> @ \<alpha>'" and elem: "(r, \<zeta>) \<in> \<delta>\<epsilon> M q X"
+    using step\<^sub>1_rule_ext[of q "[]" \<alpha> r u \<beta>] by blast
+  from 2(4)[of r \<beta>] have "r \<notin> final_states M"
+    using step\<^sub>1_steps[OF 2(1)[unfolded u_def]] by simp
+  with elem have "(S2 r, \<zeta>) \<in> comp_dpda_delta_eps (S2 q) X" by force
+  with \<alpha>_def * have **: "(S2 q, [], \<alpha>) \<leadsto>\<^sub>c (S2 r, [], \<beta>)"
+    using comp.step\<^sub>1_rule[of "S2 q" "[]" X \<alpha>' "S2 r" "[]" \<beta>] by (simp add: comp_dpda_def)
+  from 2(4) have nr: "\<And>s \<mu>. (r, [], \<beta>) \<leadsto>* (s, [], \<mu>) \<longrightarrow> s \<notin> final_states M"
+    using steps_trans[OF step\<^sub>1_steps[OF 2(1)], unfolded u_def] by blast
+  from 2(3)[OF u_def nr] have ***: "(S2 r, [], \<beta>) \<leadsto>\<^sub>c* (S2 p, [], \<gamma>)" .
+  show ?case
+    using comp.steps_trans[OF comp.step\<^sub>1_steps[OF **] ***] .
+qed
 
-(* Combinations 
-                 h1 h2
-                 h3 h4
-                 h1 h3
-                 h2 h4 *)
+text \<open>The automaton @{const [source] comp_dpda} mimics the steps of the original automaton in S2-states, 
+      provided that the word read so far is not accepted:\<close>
+lemma comp_dpda_nonfinal_steps:
+  assumes "(q', w, \<alpha>) \<leadsto>* (p, u, \<gamma>)"
+      and "w \<noteq> u"
+      and "\<And>r \<beta>. (q', w, \<alpha>) \<leadsto>* (r, u, \<beta>) \<longrightarrow> r \<notin> final_states M"
+      and "q = S1 q' \<or> q = S2 q'"
+    shows "(q, w, \<alpha>) \<leadsto>\<^sub>c* (S2 p, u, \<gamma>)"
+using assms proof (induction "(q', w, \<alpha>)" "(p, u, \<gamma>)" arbitrary: q q' w \<alpha> rule: steps_induct2)
+  case (2 q' w \<alpha> r v \<beta>)
+  from 2(1) obtain X \<alpha>' where \<alpha>_def: "\<alpha> = X#\<alpha>'" and cases:
+      "(\<exists>\<zeta>. v = w \<and> \<beta> = \<zeta> @ \<alpha>' \<and> (r, \<zeta>) \<in> \<delta>\<epsilon> M q' X) \<or> (\<exists>a \<zeta>. w = a # v \<and> \<beta> = \<zeta> @ \<alpha>' \<and> (r, \<zeta>) \<in> \<delta> M q' a X)" (is "?a \<or> ?b")
+    using step\<^sub>1_rule_ext[of q' w \<alpha> r v \<beta>] by blast
+  from 2(5) have rp_nonfinal: "\<And>ra \<beta>'. (r, v, \<beta>) \<leadsto>* (ra, u, \<beta>') \<longrightarrow> ra \<notin> final_states M"
+      using steps_trans[OF step\<^sub>1_steps[OF 2(1)]] by blast
+  from cases consider (a) ?a | (b) ?b by blast
+  then show ?case
+  proof cases
+    case a
+    then obtain \<zeta> where *: "v = w" and **: "\<beta> = \<zeta> @ \<alpha>'" and elem: "(r, \<zeta>) \<in> \<delta>\<epsilon> M q' X" by blast
+    from elem 2(6) have "(S1 r, \<zeta>) \<in> comp_dpda_delta_eps q X \<or> (S2 r, \<zeta>) \<in> comp_dpda_delta_eps q X" by force
+    with * ** \<alpha>_def have ***: "(q, w, \<alpha>) \<leadsto>\<^sub>c (S1 r, v, \<beta>) \<or> (q, w, \<alpha>) \<leadsto>\<^sub>c (S2 r, v, \<beta>)"
+      using comp.step\<^sub>1_rule[of q w X \<alpha>' _ v \<beta>] by (simp add: comp_dpda_def)
+    from 2(4) * have v_neq: "v \<noteq> u" by simp
+    from 2(3)[OF v_neq rp_nonfinal] have ****: "(S1 r, v, \<beta>) \<leadsto>\<^sub>c* (S2 p, u, \<gamma>)" by simp
+    from 2(3)[OF v_neq rp_nonfinal] have *****: "(S2 r, v, \<beta>) \<leadsto>\<^sub>c* (S2 p, u, \<gamma>)" by simp
+    from *** **** ***** show ?thesis
+      using comp.step\<^sub>1_steps comp.steps_trans by blast
+  next
+    case b
+    then obtain a \<zeta> where *: "w = a # v" and **: "\<beta> = \<zeta> @ \<alpha>'" and elem: "(r, \<zeta>) \<in> \<delta> M q' a X" by blast
+    show ?thesis
+    proof (cases "v = u")
+      case True
+      from 2(5) have r_nonfinal: "r \<notin> final_states M"
+        using step\<^sub>1_steps[OF 2(1)[unfolded True]] by simp
+      from 2(6) consider (s1) "q = S1 q'" | (s2) "q = S2 q'" by blast
+      then have p1: "(q, w, \<alpha>) \<leadsto>\<^sub>c* (S2 r, v, \<beta>)"
+      proof cases
+        case s1
+        with elem r_nonfinal have "(S2 r, \<zeta>) \<in> comp_dpda_delta q a X" by force
+        with * ** \<alpha>_def have ***: "(q, w, \<alpha>) \<leadsto>\<^sub>c (S2 r, v, \<beta>)"
+          using comp.step\<^sub>1_rule[of q w X \<alpha>' "S2 r" v \<beta>] by (simp add: comp_dpda_def)
+        show ?thesis
+          using comp.step\<^sub>1_steps[OF ***] .
+      next
+        case s2
+        with elem have "(S3 q', [X]) \<in> comp_dpda_delta_eps q X" by auto
+        with \<alpha>_def have ***: "(q, w, \<alpha>) \<leadsto>\<^sub>c (S3 q', w, \<alpha>)"
+          using comp.step\<^sub>1_rule[of q w X \<alpha>' "S3 q'" w \<alpha>] by (simp add: comp_dpda_def)
+        from elem r_nonfinal have "(S2 r, \<zeta>) \<in> comp_dpda_delta (S3 q') a X" by force
+        with * ** \<alpha>_def have ****: "(S3 q', w, \<alpha>) \<leadsto>\<^sub>c (S2 r, v, \<beta>)"
+          using comp.step\<^sub>1_rule[of "S3 q'" w X \<alpha>' "S2 r" v \<beta>] by (simp add: comp_dpda_def)
+        show ?thesis
+          using comp.steps_trans[OF comp.step\<^sub>1_steps[OF ***] comp.step\<^sub>1_steps[OF ****]] .
+      qed
+      from 2(2)[unfolded True] have a1: "(r, [], \<beta>) \<leadsto>* (p, [], \<gamma>)" 
+        using steps_word_app[of r "[]" \<beta> p "[]" \<gamma> u] by simp
+      from rp_nonfinal[unfolded True] have a2: "\<And>ra \<beta>'. (r, [], \<beta>) \<leadsto>* (ra, [], \<beta>') \<longrightarrow> ra \<notin> final_states M"
+        using steps_word_app[of r "[]" \<beta> _ "[]" _ u] by simp
+      have "(S2 r, [], \<beta>) \<leadsto>\<^sub>c* (S2 p, [], \<gamma>)"
+        using comp_dpda_nonfinal_stepsS2[OF a1 a2] .
+      with True have p2: "(S2 r, v, \<beta>) \<leadsto>\<^sub>c* (S2 p, u, \<gamma>)"
+        using comp.steps_word_app[of "S2 r" "[]" \<beta> "S2 p" "[]" \<gamma> u] by simp
+      show ?thesis
+        using comp.steps_trans[OF p1 p2] .
+    next
+      case False
+      from 2(6) consider (s1) "q = S1 q'" | (s2) "q = S2 q'" by blast
+      then have p: "(q, w, \<alpha>) \<leadsto>\<^sub>c* (S1 r, v, \<beta>) \<or> (q, w, \<alpha>) \<leadsto>\<^sub>c* (S2 r, v, \<beta>)"
+      proof (cases)
+        case s1
+        with elem have "(S1 r, \<zeta>) \<in> comp_dpda_delta q a X \<or> (S2 r, \<zeta>) \<in> comp_dpda_delta q a X" by force
+        with * ** \<alpha>_def have "(q, w, \<alpha>) \<leadsto>\<^sub>c (S1 r, v, \<beta>) \<or> (q, w, \<alpha>) \<leadsto>\<^sub>c (S2 r, v, \<beta>)"
+          using comp.step\<^sub>1_rule[of q w X \<alpha>' _ v \<beta>] by (simp add: comp_dpda_def)
+        then show ?thesis
+          using comp.step\<^sub>1_steps by blast
+      next
+        case s2
+        with elem have "(S3 q', [X]) \<in> comp_dpda_delta_eps q X" by auto
+        with \<alpha>_def have ***: "(q, w, \<alpha>) \<leadsto>\<^sub>c (S3 q', w, \<alpha>)"
+          using comp.step\<^sub>1_rule[of q w X \<alpha>' "S3 q'" w \<alpha>] by (simp add: comp_dpda_def)
+        from elem have "(S1 r, \<zeta>) \<in> comp_dpda_delta (S3 q') a X \<or> (S2 r, \<zeta>) \<in> comp_dpda_delta (S3 q') a X" by force
+        with * ** \<alpha>_def have ****: "(S3 q', w, \<alpha>) \<leadsto>\<^sub>c (S1 r, v, \<beta>) \<or> (S3 q', w, \<alpha>) \<leadsto>\<^sub>c (S2 r, v, \<beta>)"
+          using comp.step\<^sub>1_rule[of "S3 q'" w X \<alpha>' _ v \<beta>] by (simp add: comp_dpda_def)
+        from *** **** show ?thesis
+          using comp.step\<^sub>1_steps comp.steps_trans by metis
+      qed
+      from 2(3)[OF False rp_nonfinal] have p1: "(S1 r, v, \<beta>) \<leadsto>\<^sub>c* (S2 p, u, \<gamma>)" by simp
+      from 2(3)[OF False rp_nonfinal] have p2: "(S2 r, v, \<beta>) \<leadsto>\<^sub>c* (S2 p, u, \<gamma>)" by simp
+      from p p1 p2 show ?thesis
+        using comp.steps_trans by blast
+    qed
+  qed
+qed simp
 
-(* TODO *)
-lemma "comp.accept_final = UNIV - accept_final"
-  sorry
+text \<open>The automaton @{const [source] comp_dpda} transitions to an S1-state if the target state is a final state:\<close>
+lemma comp_dpda_final_steps:
+  assumes "(q', w, \<alpha>) \<leadsto>+ (p, u, \<gamma>)"
+      and "p \<in> final_states M"
+      and "q = S1 q' \<or> q = S2 q'"
+    shows "(q, w, \<alpha>) \<leadsto>\<^sub>c+ (S1 p, u, \<gamma>)"
+using assms proof (induction "(q', w, \<alpha>)" "(p, u, \<gamma>)" arbitrary: q q' w \<alpha> rule: stepst_induct2)
+  case (1 q' w \<alpha>)
+  from 1(1) obtain X \<alpha>' where \<alpha>_def: "\<alpha> = X#\<alpha>'" and cases:
+      "(\<exists>\<beta>. u = w \<and> \<gamma> = \<beta> @ \<alpha>' \<and> (p, \<beta>) \<in> \<delta>\<epsilon> M q' X) \<or> (\<exists>a \<beta>. w = a # u \<and> \<gamma> = \<beta> @ \<alpha>' \<and> (p, \<beta>) \<in> \<delta> M q' a X)" (is "?a \<or> ?b")
+    using step\<^sub>1_rule_ext[of q' w \<alpha> p u \<gamma>] by blast
+  from cases consider (a) ?a | (b) ?b by blast
+  then show ?case
+  proof cases
+    case a
+    then obtain \<beta> where *: "u = w" and **: "\<gamma> = \<beta> @ \<alpha>'" and elem: "(p, \<beta>) \<in> \<delta>\<epsilon> M q' X" by blast
+    from 1(2,3) elem have "(S1 p, \<beta>) \<in> comp_dpda_delta_eps q X" by force
+    with * ** \<alpha>_def have ***: "(q, w, \<alpha>) \<leadsto>\<^sub>c (S1 p, u, \<gamma>)"
+      using comp.step\<^sub>1_rule[of q w X \<alpha>' "S1 p" u \<gamma>] by (simp add: comp_dpda_def)
+    show ?thesis
+      using comp.stepst_step[OF ***] .
+  next
+    case b
+    then obtain a \<beta> where *: "w = a # u" and **: "\<gamma> = \<beta> @ \<alpha>'" and elem: "(p, \<beta>) \<in> \<delta> M q' a X" by blast
+    from 1(3) consider (c) "q = S1 q'" | (d) "q = S2 q'" by blast
+    then show ?thesis
+    proof cases
+      case c
+      with elem 1(2) have "(S1 p, \<beta>) \<in> comp_dpda_delta q a X" by force
+      with * ** \<alpha>_def have ***: "(q, w, \<alpha>) \<leadsto>\<^sub>c (S1 p, u, \<gamma>)"
+        using comp.step\<^sub>1_rule[of q w X \<alpha>' "S1 p" u \<gamma>] by (simp add: comp_dpda_def)
+      show ?thesis
+        using comp.stepst_step[OF ***] .
+    next
+      case d
+      with elem have "(S3 q', [X]) \<in> comp_dpda_delta_eps q X" by auto
+      with \<alpha>_def have ***: "(q, w, \<alpha>) \<leadsto>\<^sub>c (S3 q', w, \<alpha>)"
+        using comp.step\<^sub>1_rule[of q w X \<alpha>' "S3 q'" w \<alpha>] by (simp add: comp_dpda_def)
+      from elem 1(2) have "(S1 p, \<beta>) \<in> comp_dpda_delta (S3 q') a X" by force
+      with * ** \<alpha>_def have ****: "(S3 q', w, \<alpha>) \<leadsto>\<^sub>c (S1 p, u, \<gamma>)"
+        using comp.step\<^sub>1_rule[of "S3 q'" w X \<alpha>' "S1 p" u \<gamma>] by (simp add: comp_dpda_def)
+      show ?thesis
+        using comp.stepst_trans[OF comp.stepst_step[OF ***] comp.stepst_step[OF ****]] .
+    qed
+  qed
+next
+  case (2 q' w \<alpha> r v \<beta>)
+  from 2(1) obtain X \<alpha>' where \<alpha>_def: "\<alpha> = X#\<alpha>'" and cases:
+      "(\<exists>\<beta>'. v = w \<and> \<beta> = \<beta>' @ \<alpha>' \<and> (r, \<beta>') \<in> \<delta>\<epsilon> M q' X) \<or> (\<exists>a \<beta>'. w = a # v \<and> \<beta> = \<beta>' @ \<alpha>' \<and> (r, \<beta>') \<in> \<delta> M q' a X)" (is "?c \<or> ?d")
+    using step\<^sub>1_rule_ext[of q' w \<alpha> r v \<beta>] by blast
+  from 2(5) consider (a) "q = S1 q'" | (b) "q = S2 q'" by blast
+  then show ?case
+  proof cases
+    case a
+    from cases consider (c) ?c | (d) ?d by blast
+    then show ?thesis
+    proof cases
+      case c
+      then obtain \<zeta> where *: "v = w" and **: "\<beta> = \<zeta> @ \<alpha>'" and elem: "(r, \<zeta>) \<in> \<delta>\<epsilon> M q' X" by blast
+      from elem a have "(S1 r, \<zeta>) \<in> comp_dpda_delta_eps q X" by auto
+      with * ** \<alpha>_def have ***: "(q, w, \<alpha>) \<leadsto>\<^sub>c (S1 r, v, \<beta>)"
+        using comp.step\<^sub>1_rule[of q w X \<alpha>' "S1 r" v \<beta>] by (simp add: comp_dpda_def)
+      from 2(3)[OF 2(4)] have ****: "(S1 r, v, \<beta>) \<leadsto>\<^sub>c+ (S1 p, u, \<gamma>)" by simp
+      show ?thesis
+        using comp.stepst_trans[OF comp.stepst_step[OF ***] ****] .
+    next
+      case d
+      then obtain a \<zeta> where *: "w = a # v" and **: "\<beta> = \<zeta> @ \<alpha>'" and elem: "(r, \<zeta>) \<in> \<delta> M q' a X" by blast
+      from elem a have "(S1 r, \<zeta>) \<in> comp_dpda_delta q a X \<or> (S2 r, \<zeta>) \<in> comp_dpda_delta q a X" by force
+      with * ** \<alpha>_def have ***: "(q, w, \<alpha>) \<leadsto>\<^sub>c (S1 r, v, \<beta>) \<or> (q, w, \<alpha>) \<leadsto>\<^sub>c (S2 r, v, \<beta>)"
+        using comp.step\<^sub>1_rule[of q w X \<alpha>' _ v \<beta>] by (simp add: comp_dpda_def)
+      from 2(3)[OF 2(4)] have ****: "(S1 r, v, \<beta>) \<leadsto>\<^sub>c+ (S1 p, u, \<gamma>)" by simp 
+      from 2(3)[OF 2(4)] have *****: "(S2 r, v, \<beta>) \<leadsto>\<^sub>c+ (S1 p, u, \<gamma>)" by simp
+      from *** **** ***** show ?thesis
+        using comp.stepst_step comp.stepst_trans by blast
+    qed
+  next
+    case b
+    from cases consider (c) ?c | (d) ?d by blast
+    then show ?thesis
+    proof cases
+      case c
+      then obtain \<zeta> where *: "v = w" and **: "\<beta> = \<zeta> @ \<alpha>'" and elem: "(r, \<zeta>) \<in> \<delta>\<epsilon> M q' X" by blast
+      from elem b have "(S1 r, \<zeta>) \<in> comp_dpda_delta_eps q X \<or> (S2 r, \<zeta>) \<in> comp_dpda_delta_eps q X" by force
+      with * ** \<alpha>_def have ***: "(q, w, \<alpha>) \<leadsto>\<^sub>c (S1 r, v, \<beta>) \<or> (q, w, \<alpha>) \<leadsto>\<^sub>c (S2 r, v, \<beta>)"
+        using comp.step\<^sub>1_rule[of q w X \<alpha>' _ v \<beta>] by (simp add: comp_dpda_def)
+      from 2(3)[OF 2(4)] have ****: "(S1 r, v, \<beta>) \<leadsto>\<^sub>c+ (S1 p, u, \<gamma>)" by simp 
+      from 2(3)[OF 2(4)] have *****: "(S2 r, v, \<beta>) \<leadsto>\<^sub>c+ (S1 p, u, \<gamma>)" by simp
+      from *** **** ***** show ?thesis
+        using comp.stepst_step comp.stepst_trans by blast
+    next
+      case d
+      then obtain a \<zeta> where *: "w = a # v" and **: "\<beta> = \<zeta> @ \<alpha>'" and elem: "(r, \<zeta>) \<in> \<delta> M q' a X" by blast
+      from elem b have "(S3 q', [X]) \<in> comp_dpda_delta_eps q X" by auto
+      with \<alpha>_def have ***: "(q, w, \<alpha>) \<leadsto>\<^sub>c (S3 q', w, \<alpha>)"
+        using comp.step\<^sub>1_rule[of q w X \<alpha>' "S3 q'" w \<alpha>] by (simp add: comp_dpda_def)
+      from elem have "(S1 r, \<zeta>) \<in> comp_dpda_delta (S3 q') a X \<or> (S2 r, \<zeta>) \<in> comp_dpda_delta (S3 q') a X" by force
+      with * ** \<alpha>_def have ****: "(S3 q', w, \<alpha>) \<leadsto>\<^sub>c (S1 r, v, \<beta>) \<or> (S3 q', w, \<alpha>) \<leadsto>\<^sub>c (S2 r, v, \<beta>)"
+        using comp.step\<^sub>1_rule[of "S3 q'" w X \<alpha>' _ v \<beta>] by (simp add: comp_dpda_def)
+      from 2(3)[OF 2(4)] have *****: "(S1 r, v, \<beta>) \<leadsto>\<^sub>c+ (S1 p, u, \<gamma>)" by simp
+      from 2(3)[OF 2(4)] have ******: "(S2 r, v, \<beta>) \<leadsto>\<^sub>c+ (S1 p, u, \<gamma>)" by simp
+      from *** **** ***** ****** show ?thesis
+        using comp.stepst_step comp.stepst_trans by metis
+    qed
+  qed
+qed
+
+text \<open>If the automaton @{const [source] comp_dpda} ends up in an S3-state while reading a word, 
+      then no state reached while reading that same word is final:\<close>
+lemma comp_dpda_steps_nonfinalS1:
+  assumes "(S1 q, w, \<alpha>) \<leadsto>\<^sub>c* (S3 p, [], \<gamma>)"
+      and "(q, w, \<alpha>) \<leadsto>* (r, [], \<beta>)"
+    shows "r \<notin> final_states M"
+proof
+  assume r_final: "r \<in> final_states M"
+  from assms(1) obtain n where p1: "(S1 q, w, \<alpha>) \<leadsto>\<^sub>c(n) (S3 p, [], \<gamma>)"
+    using comp.stepn_steps[of "S1 q" w \<alpha> "S3 p" "[]" \<gamma>] by blast
+  have np: "(S3 p, [], \<gamma>) \<leadsto>\<^sub>c"
+    using comp.step\<^sub>1_rule_ext[of "S3 p" "[]" \<gamma>] by (simp add: comp_dpda_def)
+  have "(S1 q, w, \<alpha>) \<leadsto>\<^sub>c* (S1 r, [], \<beta>)"
+  proof (cases "(q, w, \<alpha>) = (r, [], \<beta>)")
+    case True
+    then show ?thesis
+      by (simp add: comp.steps_refl)
+  next
+    case False
+    have q1: "(q, w, \<alpha>) \<leadsto>+ (r, [], \<beta>)"
+      using steps_stepst[OF assms(2) False] .
+    have q2: "(S1 q, w, \<alpha>) \<leadsto>\<^sub>c+ (S1 r, [], \<beta>)"
+      using comp_dpda_final_steps[OF q1 r_final] by simp
+    show ?thesis
+      using comp.stepst_steps[OF q2] .
+  qed
+  then obtain m where p2: "(S1 q, w, \<alpha>) \<leadsto>\<^sub>c(m) (S1 r, [], \<beta>)"
+    using comp.stepn_steps[of "S1 q" w \<alpha> "S1 r" "[]" \<beta>] by blast 
+  have m_leq_n: "m \<le> n"
+    using comp.max_eps_steps[OF p1 np p2] .
+  have "(S1 r, [], \<beta>) \<leadsto>\<^sub>c(n - m) (S3 p, [], \<gamma>)"
+    using comp.split_path[OF p1 m_leq_n] comp.dpda_stepn_det[OF p2] by blast
+  then have *: "(S1 r, [], \<beta>) \<leadsto>\<^sub>c* (S3 p, [], \<gamma>)"
+    using comp.stepn_steps[of "S1 r" "[]" \<beta> "S3 p" "[]" \<gamma>] by blast
+  show False
+    using comp_dpda_steps_from_S1[OF *] by simp
+qed
+
+lemma comp_dpda_steps_nonfinalS2:
+  assumes "(S2 q, w, \<alpha>) \<leadsto>\<^sub>c* (S3 p, [], \<gamma>)"
+      and "(q, w, \<alpha>) \<leadsto>+ (r, [], \<beta>)"
+    shows "r \<notin> final_states M"
+proof
+  assume r_final: "r \<in> final_states M"
+  from assms(1) obtain n where p1: "(S2 q, w, \<alpha>) \<leadsto>\<^sub>c(n) (S3 p, [], \<gamma>)"
+    using comp.stepn_steps[of "S2 q" w \<alpha> "S3 p" "[]" \<gamma>] by blast
+  have np: "(S3 p, [], \<gamma>) \<leadsto>\<^sub>c"
+    using comp.step\<^sub>1_rule_ext[of "S3 p" "[]" \<gamma>] by (simp add: comp_dpda_def)
+  obtain m where p2: "(S2 q, w, \<alpha>) \<leadsto>\<^sub>c(m) (S1 r, [], \<beta>)"
+    using comp.stepst_steps[OF comp_dpda_final_steps[OF assms(2) r_final, of "S2 q", simplified]] comp.stepn_steps[of "S2 q" w \<alpha> "S1 r" "[]" \<beta>] by blast
+  have m_leq_n: "m \<le> n"
+    using comp.max_eps_steps[OF p1 np p2] .
+  have "(S1 r, [], \<beta>) \<leadsto>\<^sub>c(n - m) (S3 p, [], \<gamma>)"
+    using comp.split_path[OF p1 m_leq_n] comp.dpda_stepn_det[OF p2] by blast
+  then have *: "(S1 r, [], \<beta>) \<leadsto>\<^sub>c* (S3 p, [], \<gamma>)"
+    using comp.stepn_steps[of "S1 r" "[]" \<beta> "S3 p" "[]" \<gamma>] by blast
+  show False
+    using comp_dpda_steps_from_S1[OF *] by simp
+qed
+
+text \<open>The language of the automaton @{const [source] comp_dpda} is the complement language:\<close>
+lemma lang_comp_dpda:
+"comp.accept_final = - accept_final"
+proof
+  show "comp.accept_final \<subseteq> - accept_final"
+  proof
+    fix w
+    assume "w \<in> comp.accept_final"
+    then obtain q \<gamma> where p: "(init_state comp_dpda, w, [init_symbol comp_dpda]) \<leadsto>\<^sub>c* (q, [], \<gamma>)" and q_final: "q \<in> final_states comp_dpda"
+      unfolding comp.accept_final_def by blast
+    from q_final obtain q' where q_def: "q = S3 q'"
+      by (auto simp: comp_dpda_def comp_dpda_final_states_def)
+    have "\<And>r \<beta>. (init_state M, w, [init_symbol M]) \<leadsto>* (r, [], \<beta>) \<longrightarrow> r \<notin> final_states M"
+    proof
+      fix r \<beta>
+      assume asm: "(init_state M, w, [init_symbol M]) \<leadsto>* (r, [], \<beta>)"
+      consider (a) "init_state M \<in> final_states M" | (b) "init_state M \<notin> final_states M" by satx
+      then show "r \<notin> final_states M"
+      proof cases
+        case a
+        with p q_def have *: "(S1 (init_state M), w, [init_symbol M]) \<leadsto>\<^sub>c* (S3 q', [], \<gamma>)"
+          by (simp add: comp_dpda_def comp_dpda_init_state_def)
+        show ?thesis
+          using comp_dpda_steps_nonfinalS1[OF * asm] .
+      next
+        case b
+        consider (c) "r = init_state M" | (d) "r \<noteq> init_state M" by satx
+        then show ?thesis
+        proof cases
+          case c
+          with b show ?thesis by simp
+        next
+          case d
+          then have *: "(init_state M, w, [init_symbol M]) \<leadsto>+ (r, [], \<beta>)"
+            using steps_stepst[OF asm] by simp
+          from b p q_def have **: "(S2 (init_state M), w, [init_symbol M]) \<leadsto>\<^sub>c* (S3 q', [], \<gamma>)"
+            by (simp add: comp_dpda_def comp_dpda_init_state_def)
+          show ?thesis
+            using comp_dpda_steps_nonfinalS2[OF ** *] .
+        qed
+      qed
+    qed
+    then show "w \<in> - accept_final"
+      by (auto simp: accept_final_def)
+  qed
+next
+  show "- accept_final \<subseteq> comp.accept_final"
+  proof
+    fix w
+    assume "w \<in> - accept_final"
+    then have nonfinal: "\<And>r \<beta>. (init_state M, w, [init_symbol M]) \<leadsto>* (r, [], \<beta>) \<longrightarrow> r \<notin> final_states M"
+      by (auto simp: accept_final_def)
+    from M_path[of w] obtain q X \<alpha> a where p: "(init_state M, w, [init_symbol M]) \<leadsto>* (q, [], X # \<alpha>)" and delta_M: "\<delta> M q a X \<noteq> {}" by blast
+    consider (a) "w = []" | (b) "w \<noteq> []" by satx
+    then have *: "(init_state comp_dpda, w, [init_symbol comp_dpda]) \<leadsto>\<^sub>c* (S2 q, [], X#\<alpha>)"
+    proof cases
+      case a
+      from nonfinal[unfolded a] have "init_state M \<notin> final_states M"
+        using steps_refl[of "init_state M" "[]" "[init_symbol M]"] by simp
+      with a show ?thesis
+        using comp_dpda_nonfinal_stepsS2[OF p[unfolded a] nonfinal[unfolded a]] by (simp add: comp_dpda_def comp_dpda_init_state_def)
+    next
+      case b
+      with p nonfinal show ?thesis
+        using comp_dpda_nonfinal_steps[of "init_state M" w "[init_symbol M]" q "[]" "X#\<alpha>"] by (simp add: comp_dpda_def comp_dpda_init_state_def)
+    qed
+    from delta_M have **: "(S2 q, [], X#\<alpha>) \<leadsto>\<^sub>c (S3 q, [], X#\<alpha>)"
+      using comp.step\<^sub>1_rule[of "S2 q" "[]" X \<alpha> "S3 q" "[]" "X#\<alpha>"] comp_dpda_def by auto
+    have "(init_state comp_dpda, w, [init_symbol comp_dpda]) \<leadsto>\<^sub>c* (S3 q, [], X # \<alpha>)"
+      using comp.steps_trans[OF * comp.step\<^sub>1_steps[OF **]] .
+    then show "w \<in> comp.accept_final"
+      using comp.accept_final_def comp_dpda_def comp_dpda_final_states_def by force
+  qed
+qed
 
 end
+
+text \<open>By constructing the two automata one after another, we get the final lemma stating that deterministic 
+      context-free languages are closed under complementation:\<close>
+lemma complement_dpda:
+  assumes "dpda (M :: ('q :: finite, 'a :: finite, 's :: finite) pda)"
+  shows "\<exists>(M' :: ('q st_extended st_num, 'a, 's sym_extended) pda). dpda M' \<and> pda.accept_final M' = - pda.accept_final M"
+proof -
+  let ?SM = "dpda_scan.scan_dpda M :: ('q st_extended, 'a, 's sym_extended) pda"
+  have dpda_sm: "dpda ?SM"
+    using assms dpda_scan.dpda_scan_dpda dpda_scan_def by blast
+  have *: "\<And>a w. \<exists>q X \<alpha>. pda.steps ?SM (init_state ?SM, w, [init_symbol ?SM]) (q, [], X#\<alpha>) \<and> delta ?SM q a X \<noteq> {}"
+    using assms dpda_scan.scan_dpda_scans dpda_scan_def by blast
+  have L1: "pda.accept_final ?SM = pda.accept_final M"
+    using assms dpda_scan.lang_scan_dpda dpda_scan.intro by auto
+  let ?CM = "complement_dpda.comp_dpda ?SM :: ('q st_extended st_num, 'a, 's sym_extended) pda"
+  from dpda_sm * have dpda_cm: "dpda ?CM"
+    using complement_dpda.dpda_comp_dpda complement_dpda.intro complement_dpda_axioms_def by blast
+  from dpda_sm * have L2: "pda.accept_final ?CM = UNIV - pda.accept_final ?SM"
+    using complement_dpda.lang_comp_dpda complement_dpda_axioms_def complement_dpda_def by blast
+  from dpda_cm L1 L2 show ?thesis by blast
+qed
+
 end
