TaskinBA/Complement/Det_Pushdown_Automata.thy
@@ -1,20 +1,12 @@
+section \<open>Deterministic Pushdown Automata\<close>
+
 theory Det_Pushdown_Automata
   imports Pushdown_Automata.Pushdown_Automata
-begin 
+begin
 
-definition the_elem_opt :: "'a set \<Rightarrow> 'a option" where
-  "the_elem_opt A \<equiv> (if A = {} then None else Some (SOME a. a : A))"
+subsection \<open>Definition\<close>
 
-text \<open>The definition @{const the_elem_opt} is intended to extract the element out of a singleton set. We will need this later as the
-      function @{const pda.step} (hopefully) produces either the empty set or a singleton set.\<close>
-
-lemma the_elem_opt_eq [simp]: "the_elem_opt {a} = Some a"
-  by (simp add: the_elem_opt_def)
-
-lemma the_elem_opt_inv: "the_elem_opt A = Some a \<Longrightarrow> a \<in> A"
-  unfolding the_elem_opt_def using some_in_eq[of A] by (auto split: if_splits)
-
-section \<open>A locale for deterministic pushdown automata\<close>
+text \<open>The following definition of a deterministic pushdown automaton has been introduced by Hopcroft and Ullman\cite{hopcroftullman}:\<close>
 
 locale dpda = pda M for M :: "('q :: finite, 'a :: finite, 's :: finite) pda" +
   assumes \<delta>_nonempty: "\<delta> M q a X \<noteq> {} \<longrightarrow> \<delta>\<epsilon> M q X = {}"
@@ -22,108 +14,55 @@ locale dpda = pda M for M :: "('q :: finite, 'a :: finite, 's :: finite) pda" +
       and \<delta>\<epsilon>_singleton: "\<delta>\<epsilon> M q X = {} \<or> (\<exists>p \<gamma>. \<delta>\<epsilon> M q X = {(p, \<gamma>)})"
 begin
 
-text \<open>In a configuration:
-      * The property @{thm \<delta>_nonempty} prevents the automaton to freely choose from an epsilon step and a true step.
-      * The property @{thm \<delta>_singleton} allows for at most one true step.
-      * The property @{thm \<delta>\<epsilon>_singleton} allows for at most one epsilon step.\<close>
+text \<open>\noindent Given a configuration:
+      \begin{itemize}
+        \item The property @{thm [source] \<delta>_nonempty} prevents the automaton to freely choose from an epsilon step and a true step.
+        \item The property @{thm [source] \<delta>_singleton} allows for at most one true step.
+        \item The property @{thm [source] \<delta>\<epsilon>_singleton} allows for at most one epsilon step.
+      \end{itemize}\<close>
 
-section \<open>Definitions\<close>
+subsection \<open>Determinism\<close>
 
-definition det_step :: "'q \<times> 'a list \<times> 's list \<Rightarrow> ('q \<times> 'a list \<times> 's list) option" where
-  "det_step cf = the_elem_opt (step cf)"
-
-abbreviation det_step\<^sub>1 ("(_ \<leadsto>\<^sub>d _)" [50, 50] 50) where
-  "cf \<leadsto>\<^sub>d cf' \<equiv> det_step cf = Some cf'"
-
-abbreviation det_nstep\<^sub>1 ("(_ \<leadsto>\<^sub>d)" [50] 50) where
-  "cf \<leadsto>\<^sub>d \<equiv>  det_step cf = None"
-
-fun det_stepn :: "nat \<Rightarrow> 'q \<times> 'a list \<times> 's list \<Rightarrow> ('q \<times> 'a list \<times> 's list) option" where
-  "det_stepn 0 cf = Some cf"
-| "det_stepn (Suc n) cf =
-    (case det_stepn n cf of None \<Rightarrow> None | Some cf' \<Rightarrow> det_step cf')"
-
-abbreviation det_stepn\<^sub>1 ("(_ /\<leadsto>\<^sub>d'(_')/ _)" [50, 0, 50] 50) where
-  "cf \<leadsto>\<^sub>d(n) cf' \<equiv> det_stepn n cf = Some cf'"
-
-abbreviation det_nstepn\<^sub>1 ("(_ /\<leadsto>\<^sub>d'(_')/ )" [50, 0] 50) where
-  "cf \<leadsto>\<^sub>d(n) \<equiv> det_stepn n cf = None"
-
-(* TODO *)
-(* (q, \<alpha>) \<leadsto> (p, \<gamma>) for (q, [], \<alpha>) \<leadsto> (p, [], \<gamma>) *)
-
-section \<open>Lemmas\<close>
-
-text \<open>The function @{const step} is indeed of deterministic nature under the locale assumptions.\<close>
-lemma dpda_step: "step (q, w, X#\<alpha>) = {} \<or> (\<exists>p u \<gamma>. step (q, w, X#\<alpha>) = {(p, u, \<gamma>)})"
-proof (cases w)
-  case Nil
-  with \<delta>\<epsilon>_singleton[of q X] 
-  show ?thesis by auto
-next
-  case [simp]: (Cons a w')
-  then show ?thesis proof (cases)
-    assume "\<delta> M q a X = {}"
-    with \<delta>\<epsilon>_singleton[of q X]
-    show ?thesis by auto
+text \<open>The automaton can take at most one step in a given configuration:\<close>
+lemma dpda_step: "step (q, w, \<alpha>) = {} \<or> (\<exists>p u \<gamma>. step (q, w, \<alpha>) = {(p, u, \<gamma>)})"
+proof (cases \<alpha>)
+  case [simp]: (Cons X \<alpha>')
+  show ?thesis proof (cases w)
+    case Nil
+    then show ?thesis
+      using \<delta>\<epsilon>_singleton[of q X] by auto
   next
-    assume a: "\<delta> M q a X \<noteq> {}"
-    from a \<delta>_singleton have *: "\<exists>p \<gamma>. \<delta> M q a X = {(p, \<gamma>)}" by auto
-    from a \<delta>_nonempty have **: "\<delta>\<epsilon> M q X = {}" by simp
-    from * ** show ?thesis by auto
+    case [simp]: (Cons a w')
+    consider (a) "\<delta> M q a X = {}" | (b) "\<delta> M q a X \<noteq> {}" by satx
+    then show ?thesis proof cases
+      case a
+      then show ?thesis
+        using \<delta>\<epsilon>_singleton[of q X] by auto
+    next
+      case b
+      then show ?thesis
+        using \<delta>_nonempty[of q a X] \<delta>_singleton[of q a X] by auto
+    qed
   qed
-qed
+qed auto
 
-text \<open>Equivalence of the definitions @{const step\<^sub>1} and @{const det_step\<^sub>1}\<close>
-lemma step\<^sub>1_det_step\<^sub>1: "(q, w, \<alpha>) \<leadsto> (p, u, \<gamma>) \<longleftrightarrow> (q, w, \<alpha>) \<leadsto>\<^sub>d (p, u, \<gamma>)" (is "?l \<longleftrightarrow> ?r")
-proof (rule iffI)
-  assume l: ?l
-  obtain X \<alpha>' where [simp]: "\<alpha> = X#\<alpha>'"
-    using step\<^sub>1_nonempty_stack[OF l] by blast
-  from l have "(p, u, \<gamma>) \<in> step (q, w, \<alpha>)" by simp
-  hence "step (q, w, \<alpha>) = {(p, u, \<gamma>)}"
-    using dpda_step[of q w X \<alpha>'] by auto
-  thus ?r by (simp add: det_step_def)
-next
-  show "?r \<Longrightarrow> ?l"
-    using the_elem_opt_inv[of "step (q, w, \<alpha>)"] by (simp add: det_step_def)
-qed
-
-text \<open>Equivalence of the definitions @{const det_step\<^sub>1} and @{const det_stepn}}}\<close>
-lemma det_step\<^sub>1_det_stepn_one: "(p\<^sub>1, w\<^sub>1, \<alpha>\<^sub>1) \<leadsto>\<^sub>d (p\<^sub>2, w\<^sub>2, \<alpha>\<^sub>2) \<longleftrightarrow> (p\<^sub>1, w\<^sub>1, \<alpha>\<^sub>1) \<leadsto>\<^sub>d(1) (p\<^sub>2, w\<^sub>2, \<alpha>\<^sub>2)"
-  by simp
-
-text \<open>A step in the automaton is deterministic.\<close>
+text \<open>A step of the automaton is indeed deterministic:\<close>
 lemma dpda_step\<^sub>1_det:
   assumes "(q, w, \<alpha>) \<leadsto> (p, u, \<gamma>)"
       and "(q, w, \<alpha>) \<leadsto> (p', u', \<gamma>')"
     shows "p = p' \<and> u = u' \<and> \<gamma> = \<gamma>'"
-using assms step\<^sub>1_det_step\<^sub>1 by simp
+using assms dpda_step by fastforce
 
-text \<open>Equivalence of the definitions @{const stepsn} and @{const det_stepn\<^sub>1}\<close>
-lemma stepn_det_stepn\<^sub>1: "(q, w, \<alpha>) \<leadsto>(n) (p, u, \<gamma>) \<longleftrightarrow> (q, w, \<alpha>) \<leadsto>\<^sub>d(n) (p, u, \<gamma>)"
-proof (induction n arbitrary: p u \<gamma>)
-  case 0
-  then show ?case by auto
-next
-  case (Suc n)
-  have "(q, w, \<alpha>) \<leadsto>(Suc n) (p, u, \<gamma>) \<longleftrightarrow> (\<exists>r v \<beta>. (q, w, \<alpha>) \<leadsto>(n) (r, v, \<beta>) \<and> (r, v, \<beta>) \<leadsto> (p, u, \<gamma>))" by auto
-  also
-  from Suc.IH have "... \<longleftrightarrow> (\<exists>r v \<beta>. (q, w, \<alpha>) \<leadsto>\<^sub>d(n) (r, v, \<beta>) \<and> (r, v, \<beta>) \<leadsto> (p, u, \<gamma>))" by simp
-  also
-  have "... \<longleftrightarrow> (\<exists>r v \<beta>. (q, w, \<alpha>) \<leadsto>\<^sub>d(n) (r, v, \<beta>) \<and> (r, v, \<beta>) \<leadsto>\<^sub>d (p, u, \<gamma>))"
-    using step\<^sub>1_det_step\<^sub>1 by simp
-  also
-  have "... \<longleftrightarrow> (q, w, \<alpha>) \<leadsto>\<^sub>d(Suc n) (p, u, \<gamma>)" by (auto split: option.split)
-  finally show ?case .
-qed
-
-text \<open>Multiple steps in the automaton are deterministic.\<close>
 lemma dpda_stepn_det:
   assumes "(q, w, \<alpha>) \<leadsto>(n) (p, u, \<gamma>)"
       and "(q, w, \<alpha>) \<leadsto>(n) (p', u', \<gamma>')"
     shows "p = p' \<and> u = u' \<and> \<gamma> = \<gamma>'"
-using assms stepn_det_stepn\<^sub>1 by simp
+using assms proof (induction "(q, w, \<alpha>)" "(p, u, \<gamma>)" arbitrary: q w \<alpha> rule: stepn_induct)
+  case (stepn n q w \<alpha> r u \<beta>)
+  from stepn(4) have *: "(r, u, \<beta>) \<leadsto>(n) (p', u', \<gamma>')"
+    using stepn_split_first[of q w \<alpha> n p' u' \<gamma>'] dpda_step\<^sub>1_det[OF stepn(1)] by auto
+  from stepn(3)[OF *] show ?case .
+qed auto
 
 end
 end
